@prefix : <https://w3.org/ns/dpv#> .
@prefix sw: <http://www.w3.org/2003/06/sw-vocab-status/ns#> .
@prefix dct: <http://purl.org/dc/terms/> .
@prefix dpv: <http://w3.org/ns/dpv#> .
@prefix owl: <http://www.w3.org/2002/07/owl#> .
@prefix rdf: <http://www.w3.org/1999/02/22-rdf-syntax-ns#> .
@prefix spl: <http://www.specialprivacy.eu/langs/usage-policy#> .
@prefix svd: <http://www.specialprivacy.eu/vocabs/data#> .
@prefix xml: <http://www.w3.org/XML/1998/namespace> .
@prefix xsd: <http://www.w3.org/2001/XMLSchema#> .
@prefix bibo: <http://purl.org/ontology/bibo/> .
@prefix prov: <http://www.w3.org/ns/prov#> .
@prefix rdfs: <http://www.w3.org/2000/01/rdf-schema#> .
@prefix svpr: <http://www.specialprivacy.eu/vocabs/processing#> .
@prefix svpu: <http://www.specialprivacy.eu/vocabs/purposes#> .
@prefix time: <http://www.w3.org/2006/time#> .
@prefix vann: <http://purl.org/vocab/vann/> .
@prefix status: <http://purl.org/ontology/bibo/status/> .
@base <https://w3.org/ns/dpv> .

<https://w3.org/ns/dpv> rdf:type owl:Ontology ;
                         dct:abstract "The Data Privacy Vocabulary provides terms (classes and properties) to annotate and categorize instances of legally compliant personal data handling according to the EU General Data Protection Regulation. This scope could be extended by later versions to other data and privacy protection regulations. The vocabulary provides terms to describe which personal data Categories are undergoing a specified kind of processing by a specific data controller and/or transferred to some recipient for a particular purpose , based on a specific legal ground (e.g. consent, or other legal grounds such as legitimate interest, etc.), with specified technical and organisational measures and restrictions (e.g. storage locations and storage durations) in place."@en ;
                         dct:contributor "Bert Bos" ,
                                         "Bud Bruegger" ,
                                         "Elmar Kiesling" ,
                                         "Eva Schlehahn" ,
                                         "Fajar J. Ekaputra" ,
                                         "Javier D. Fernández" ,
                                         "Mark Lizar" ,
                                         "Ramisa Gachpaz Hamed" ,
                                         "Rigo Wenning" ,
                                         "Rob Brennan" ,
                                         "Simon Steyskal" ;
                         dct:created "2019-06-18"^^xsd:date ;
                         dct:creator "Axel Polleres" ,
                                     "Harshvardhan J. Pandit" ;
                         dct:description "The Data Privacy Vocabulary provides terms (classes and properties) to annotate and categorize instances of legally compliant personal data handling. These terms are intended to annotate Legal Personal Data Handling in a machine-readable fashion, by specifying which personal data categories are undergoing a specific kind of processing, by a specific data controller and/or shared with some recipient for a particular purpose , based on a specific legal ground (e.g. consent or legitimate interest), with specific technical and organisational measures and restrictions (e.g. storage location and storage duration) in place."@en ;
                         dct:source <https://www.w3.org/community/dpvcg/> ;
                         dct:title "Data Privacy Vocabulary"@en ;
                         bibo:status status:draft ;
                         vann:preferredNamespacePrefix "dpv" ;
                         vann:preferredNamespaceUri "https://w3.org/ns/dpv"^^xsd:string ;
                         owl:versionInfo "0.1"^^xsd:string .

#################################################################
#    Annotation properties
#################################################################

###  http://purl.org/dc/terms/abstract
dct:abstract rdf:type owl:AnnotationProperty .


###  http://purl.org/dc/terms/contributor
dct:contributor rdf:type owl:AnnotationProperty .


###  http://purl.org/dc/terms/created
dct:created rdf:type owl:AnnotationProperty .


###  http://purl.org/dc/terms/creator
dct:creator rdf:type owl:AnnotationProperty .


###  http://purl.org/dc/terms/date-accepted
dct:date-accepted rdf:type owl:AnnotationProperty .


###  http://purl.org/dc/terms/description
dct:description rdf:type owl:AnnotationProperty .


###  http://purl.org/dc/terms/modified
dct:modified rdf:type owl:AnnotationProperty .


###  http://purl.org/dc/terms/source
dct:source rdf:type owl:AnnotationProperty .


###  http://purl.org/dc/terms/title
dct:title rdf:type owl:AnnotationProperty .


###  http://purl.org/ontology/bibo/status
bibo:status rdf:type owl:AnnotationProperty .


###  http://purl.org/vocab/vann/preferredNamespacePrefix
vann:preferredNamespacePrefix rdf:type owl:AnnotationProperty .


###  http://purl.org/vocab/vann/preferredNamespaceUri
vann:preferredNamespaceUri rdf:type owl:AnnotationProperty .


###  http://w3.org/ns/dpv#consentNotice
dpv:consentNotice rdf:type owl:AnnotationProperty ;
                  dct:created "2019-04-04"^^xsd:date ;
                  dct:creator "Harshvardhan J. Pandit, Mark Lizar, Bud Bruegger" ;
                  dct:date-accepted "2019-04-05"^^xsd:date ;
                  dct:description "Links consent to the notice displayed for requesting consent"@en ;
                  rdfs:comment "The actual notice that the Data Subject received to consent to, either a text or link to a document, which should be usable to decide whether the form or consent was compliant to legislation, e.g. documenting how the user has been informed about rights and implications (such as, right to data portability,right to recitffy, right to erasure, right to restrict processing, right to object, rights regarding automated decision making or profiling, processors, third parties, sub-processors, outside-EEA transfers, automated decision-making, or other necessary details of the privacy-policy). Can be TextOrDocumentOrURI." ;
                  sw:term_status "accepted" ;
                  rdfs:domain dpv:Consent .


###  http://w3.org/ns/dpv#expiry
dpv:expiry rdf:type owl:AnnotationProperty ;
           dct:created "2019-04-04"^^xsd:date ;
           dct:creator "Harshvardhan J. Pandit, Mark Lizar, Bud Bruegger" ;
           dct:date-accepted "2019-04-05"^^xsd:date ;
           dct:description "Generic property specifying when or under which condition(s) the consent will expire"@en ;
           sw:term_status "accepted" ;
           rdfs:domain dpv:Consent .


###  http://w3.org/ns/dpv#expiryCondition
dpv:expiryCondition rdf:type owl:AnnotationProperty ;
                    dct:created "2019-04-04"^^xsd:date ;
                    dct:creator "Harshvardhan J. Pandit, Mark Lizar, Bud Bruegger" ;
                    dct:date-accepted "2019-04-05"^^xsd:date ;
                    dct:description "Specifies the condition or event that determines the expiry of consent"@en ;
                    rdfs:comment "Can be TextOrDocumentOrURI" ;
                    sw:term_status "accepted" ;
                    rdfs:domain dpv:Consent .


###  http://w3.org/ns/dpv#innovativeUseOfNewSolutions
dpv:innovativeUseOfNewSolutions rdf:type owl:AnnotationProperty ;
                                dct:created "2019-04-04"^^xsd:date ;
                                dct:date-accepted "2019-05-07"^^xsd:date ;
                                dct:description "Indicates the processing comprises of innovative uses of new or radical solutions"@en ;
                                rdfs:comment "e.g. combining fingerprint & face scan for access control. What is concidered new/innovative is of course subject to change over time." ;
                                rdfs:isDefinedBy "DPVCG" ;
                                sw:term_status "accepted" ;
                                rdfs:domain dpv:Processing .


###  http://w3.org/ns/dpv#isAutomatedDecisionMaking
dpv:isAutomatedDecisionMaking rdf:type owl:AnnotationProperty ;
                              dct:created "2019-04-04"^^xsd:date ;
                              dct:date-accepted "2019-05-07"^^xsd:date ;
                              dct:description "Indicates whether the processing comprises of or is part of or results in automated decision making"@en ;
                              rdfs:isDefinedBy "DPVCG" ;
                              sw:term_status "accepted" ;
                              rdfs:domain dpv:Processing .


###  http://w3.org/ns/dpv#isEvaluationScoring
dpv:isEvaluationScoring rdf:type owl:AnnotationProperty ;
                        dct:created "2019-04-04"^^xsd:date ;
                        dct:date-accepted "2019-05-07"^^xsd:date ;
                        dct:description "Indicates whether the processing ir part of or results in evaluation or scoring of an individual or their personal data"@en ;
                        rdfs:comment "including profiling and predicting," ;
                        rdfs:isDefinedBy "DPVCG" ;
                        sw:term_status "accepted" ;
                        rdfs:domain dpv:Processing .


###  http://w3.org/ns/dpv#isExplicit
dpv:isExplicit rdf:type owl:AnnotationProperty ;
               dct:created "2019-04-04"^^xsd:date ;
               dct:creator "Harshvardhan J. Pandit, Mark Lizar, Bud Bruegger" ;
               dct:date-accepted "2019-04-05"^^xsd:date ;
               dct:description "Indicates consent is explicit as explained in GDPR Article 9.2a and Article 22.2c"@en ;
               sw:term_status "accepted" ;
               rdfs:domain dpv:Consent .


###  http://w3.org/ns/dpv#isLargeScale
dpv:isLargeScale rdf:type owl:AnnotationProperty ;
                 dct:created "2019-04-04"^^xsd:date ;
                 dct:date-accepted "2019-05-07"^^xsd:date ;
                 dct:description "Indicates the processing is carried out at large scale in terms of size of data or individuals associated"@en ;
                 rdfs:comment "Involves large amounts of personal data or data subjects. The WP29 recommends that the following factors, in particular, be considered when determining whether the processing is carried out on a large scale (WP29 Guidelines on Data Protection Officer 16/EN WP 243): a. the number of data subjects concerned, either as a specific number or as a proportion of the relevant population; b. the volume of data and/or the range of different data items being processed; c. the duration, or permanence, of the data processing activity; d. the geographical extent of the processing activity." ;
                 rdfs:isDefinedBy "DPVCG" ;
                 sw:term_status "accepted" ;
                 rdfs:domain dpv:Processing .


###  http://w3.org/ns/dpv#isMatchingCombining
dpv:isMatchingCombining rdf:type owl:AnnotationProperty ;
                        dct:created "2019-04-04"^^xsd:date ;
                        dct:date-accepted "2019-05-07"^^xsd:date ;
                        dct:description "Indicates whether the processing comprises of matching or combining existing data"@en ;
                        rdfs:comment "originating from two or more data processing operations performed for different purposes and/or by different data controllers in a way that would exceed the reasonable expectations of the data subject (WP29 Opinion on Purpose limitation 13/EN WP 203, p.24).  For instance Integration/Enrichment with other data (not necessarily personal only)" ;
                        rdfs:isDefinedBy "DPVCG" ;
                        sw:term_status "accepted" ;
                        rdfs:domain dpv:Processing .


###  http://w3.org/ns/dpv#isSystematicMonitoring
dpv:isSystematicMonitoring rdf:type owl:AnnotationProperty ;
                           dct:created "2019-04-04"^^xsd:date ;
                           dct:date-accepted "2019-05-07"^^xsd:date ;
                           dct:description "Indicates whether the processing comprises of systematic monitoring of data subjects or their personal data"@en ;
                           rdfs:isDefinedBy "DPVCG" ;
                           sw:term_status "accepted" ;
                           rdfs:domain dpv:Processing .


###  http://w3.org/ns/dpv#measureImplementedBy
dpv:measureImplementedBy rdf:type owl:AnnotationProperty ;
                         dct:created "2019-04-23"^^xsd:date ;
                         dct:creator "Axel Polleres" ;
                         dct:date-accepted "2019-05-07"^^xsd:date ;
                         dct:description "a generic ObjectProperty to describe how the measure is implemented.  For the values of this property we either allow a blank node with a single rdfs:comment to describe the measure, or a URI to a standard or best practice followed, i.e. a well-known identifier for that standard or a URL where the respective document describes the standard."@en ;
                         rdfs:isDefinedBy "DPVCG" ;
                         sw:term_status "accepted" ;
                         rdfs:domain dpv:TechnicalOrganisationalMeasure .


###  http://w3.org/ns/dpv#provisionByJustification
dpv:provisionByJustification rdf:type owl:AnnotationProperty ;
                             dct:created "2019-04-04"^^xsd:date ;
                             dct:creator "Harshvardhan J. Pandit, Mark Lizar, Bud Bruegger" ;
                             dct:date-accepted "2019-04-05"^^xsd:date ;
                             dct:description "Specifies the justification for entity providing consent"@en ;
                             rdfs:comment "This field can be used to proivde a justification why the provision was provided by another DataSubject or legal entity,  e.g. declariing the relationship (parent, guardian), in combination with the field provisionBy" ;
                             sw:term_status "accepted" ;
                             rdfs:domain dpv:Consent .


###  http://w3.org/ns/dpv#provisionMethod
dpv:provisionMethod rdf:type owl:AnnotationProperty ;
                    dct:created "2019-04-04"^^xsd:date ;
                    dct:creator "Harshvardhan J. Pandit, Mark Lizar, Bud Bruegger" ;
                    dct:date-accepted "2019-04-05"^^xsd:date ;
                    dct:description "Specifies the method by which consent was provisioned or provided"@en ;
                    rdfs:comment "Can be used to record information of how consent was provided e.g. by a click to a form, in writing, etc., by logging into a system and confirm per email, or with some additional authentication, etc." ;
                    sw:term_status "accepted" ;
                    rdfs:domain dpv:Consent .


###  http://w3.org/ns/dpv#withdrawalByJustification
dpv:withdrawalByJustification rdf:type owl:AnnotationProperty ;
                              dct:created "2019-04-04"^^xsd:date ;
                              dct:creator "Harshvardhan J. Pandit, Mark Lizar, Bud Bruegger" ;
                              dct:date-accepted "2019-04-05"^^xsd:date ;
                              dct:description "Specifies the justification for entity withdrawing consent"@en ;
                              rdfs:comment "This field can be used to proivde a justification why the weithdrawal was done by another DataSubject or legal entity, e.g. declariing the relationship (parent, guardian), in combination with the field withdrawalBy" ;
                              sw:term_status "accepted" ;
                              rdfs:domain dpv:Consent .


###  http://w3.org/ns/dpv#withdrawalMethod
dpv:withdrawalMethod rdf:type owl:AnnotationProperty ;
                     dct:created "2019-04-04"^^xsd:date ;
                     dct:creator "Harshvardhan J. Pandit, Mark Lizar, Bud Bruegger" ;
                     dct:date-accepted "2019-04-05"^^xsd:date ;
                     dct:description "Specifries the method by which consent can be/has been withdrawn"@en ;
                     rdfs:comment "Can be used to record information of how to withdraw consent, e.g. by a click to a form, in writing, etc., by logging into a system and confirm per email, or with some additional authentication, etc." ;
                     sw:term_status "accepted" ;
                     rdfs:domain dpv:Consent .


###  http://www.w3.org/2003/06/sw-vocab-status/ns#term_status
sw:term_status rdf:type owl:AnnotationProperty .


#################################################################
#    Datatypes
#################################################################

###  http://www.w3.org/2001/XMLSchema#date
xsd:date rdf:type rdfs:Datatype .


#################################################################
#    Object Properties
#################################################################

###  http://w3.org/ns/dpv#duration
dpv:duration rdf:type owl:ObjectProperty ;
             rdfs:domain dpv:StorageRestriction ;
             rdfs:range dpv:StorageDuration ;
             dct:created "2019-04-04"^^xsd:date ;
             dct:creator "Axel Polleres, Rob Brennan, Harshvardhan J. Pandit, Mark Lizar" ;
             dct:date-accepted "2019-04-05"^^xsd:date ;
             dct:description "Specifies duration for storage of personal data"@en ;
             rdfs:isDefinedBy "DPVCG" ;
             sw:term_status "accepted" .


###  http://w3.org/ns/dpv#expiryTime
dpv:expiryTime rdf:type owl:ObjectProperty ;
               rdfs:domain dpv:Consent ;
               rdfs:range time:TemporalEntity ;
               dct:created "2019-04-04"^^xsd:date ;
               dct:creator "Harshvardhan J. Pandit, Mark Lizar, Bud Bruegger" ;
               dct:date-accepted "2019-04-05"^^xsd:date ;
               dct:description "Specifies the expiry time or duration for consent"@en ;
               sw:term_status "accepted" .


###  http://w3.org/ns/dpv#hasBeneficiary
dpv:hasBeneficiary rdf:type owl:ObjectProperty ;
                   rdfs:domain dpv:Context ;
                   rdfs:range dpv:Beneficiary ;
                   dct:created "2019-05-23"^^xsd:date ;
                   dct:description "Cui bono? Who is the ultimate beneficiary of this purpose, here a stakeholder can be declared, e.g. the DataSubjects themselves or the Data Controller. ( --- under consideration --- )"@en ;
                   sw:term_status "proposed" .


###  http://w3.org/ns/dpv#hasContext
dpv:hasContext rdf:type owl:ObjectProperty ;
               rdfs:domain dpv:Purpose ;
               rdfs:range dpv:Context ;
               dct:created "2019-04-04"^^xsd:date ;
               dct:date-accepted "2019-04-05"^^xsd:date ;
               dct:description "Restricts a purpose to the specified context(s)"@en ;
               sw:term_status "accepted" .


###  http://w3.org/ns/dpv#hasDataController
dpv:hasDataController rdf:type owl:ObjectProperty ;
                      rdfs:range dpv:DataController ;
                      dct:created "2019-04-04"^^xsd:date ;
                      dct:creator "Axel Polleres, Javier Ferenandez, Harshvardhan J. Pandit, Mark Lizar, Bud Bruegger" ;
                      dct:date-accepted "2019-04-05"^^xsd:date ;
                      dct:description "This property associates a data controller with an instance of legal data handling or consent"@en ;
                      rdfs:comment "We replicate all the properties except Legalbasis of personal data handling for consent, to declare what kinds of personal data handling are consented to" ;
                      rdfs:isDefinedBy "DPVCG" ;
                      sw:term_status "accepted" .


###  http://w3.org/ns/dpv#hasDataSubject
dpv:hasDataSubject rdf:type owl:ObjectProperty ;
                   rdfs:range dpv:DataSubject ;
                   dct:created "2019-04-04"^^xsd:date ;
                   dct:creator "Axel Polleres, Javier Ferenandez, Harshvardhan J. Pandit, Mark Lizar, Bud Bruegger" ;
                   dct:date-accepted "2019-04-05"^^xsd:date ;
                   dct:description "This property associates a data subject with an instance of legal data handling or consent"@en ;
                   rdfs:comment "We replicate all the properties except Legalbasis of personal data handling for consent, to declare what kinds of personal data handling are consented to" ;
                   rdfs:isDefinedBy "DPVCG" ;
                   sw:term_status "accepted" .


###  http://w3.org/ns/dpv#hasLegalBasis
dpv:hasLegalBasis rdf:type owl:ObjectProperty ;
                  rdfs:domain dpv:PersonalDataHandling ;
                  rdfs:range dpv:LegalBasis ;
                  dct:created "2019-04-04"^^xsd:date ;
                  dct:creator "Axel Polleres, Javier Ferenandez" ;
                  dct:date-accepted "2019-04-05"^^xsd:date ;
                  dct:description "This property associates an instance of legal data handling with its underlying legal basis"@en ;
                  rdfs:isDefinedBy "DPVCG" ;
                  sw:term_status "accepted" .


###  http://w3.org/ns/dpv#hasPersonalDataCategory
dpv:hasPersonalDataCategory rdf:type owl:ObjectProperty ;
                            rdfs:range dpv:PersonalDataCategory ;
                            dct:created "2019-04-04"^^xsd:date ;
                            dct:creator "Axel Polleres, Javier Ferenandez, Harshvardhan J. Pandit, Mark Lizar, Bud Bruegger" ;
                            dct:date-accepted "2019-04-05"^^xsd:date ;
                            dct:description "This property associates a personal data category with an instance of legal data handling or consent"@en ;
                            rdfs:comment "We replicate all the properties except Legalbasis of personal data handling for consent, to declare what kinds of personal data handling are consented to" ;
                            rdfs:isDefinedBy "DPVCG" ;
                            sw:term_status "accepted" .


###  http://w3.org/ns/dpv#hasProcessing
dpv:hasProcessing rdf:type owl:ObjectProperty ;
                  rdfs:range dpv:Processing ;
                  dct:created "2019-04-04"^^xsd:date ;
                  dct:creator "Axel Polleres, Javier Ferenandez, Harshvardhan J. Pandit, Mark Lizar, Bud Bruegger" ;
                  dct:date-accepted "2019-04-05"^^xsd:date ;
                  dct:description "This property associates a data processing category with an instance of legal data handling or consent"@en ;
                  rdfs:comment "We replicate all the properties except Legalbasis of personal data handling for consent, to declare what kinds of personal data handling are consented to" ;
                  rdfs:isDefinedBy "DPVCG" ;
                  sw:term_status "accepted" .


###  http://w3.org/ns/dpv#hasPurpose
dpv:hasPurpose rdf:type owl:ObjectProperty ;
               rdfs:range dpv:Purpose ;
               dct:created "2019-04-04"^^xsd:date ;
               dct:creator "Axel Polleres, Javier Ferenandez, Harshvardhan J. Pandit, Mark Lizar, Bud Bruegger" ;
               dct:date-accepted "2019-04-05"^^xsd:date ;
               dct:description "This property associates a purpose with an instance of legal data handling or consent"@en ;
               rdfs:comment "We replicate all the properties except Legalbasis of personal data handling for consent, to declare what kinds of personal data handling are consented to" ;
               rdfs:isDefinedBy "DPVCG" ;
               sw:term_status "accepted" .


###  http://w3.org/ns/dpv#hasRecipient
dpv:hasRecipient rdf:type owl:ObjectProperty ;
                 rdfs:range dpv:Recipient ;
                 dct:created "2019-04-04"^^xsd:date ;
                 dct:creator "Axel Polleres, Javier Ferenandez, Harshvardhan J. Pandit, Mark Lizar, Bud Bruegger" ;
                 dct:date-accepted "2019-04-05"^^xsd:date ;
                 dct:description "This property associates a recipient with an instance of legal data handling or consent"@en ;
                 rdfs:comment "We replicate all the properties except Legalbasis of personal data handling for consent, to declare what kinds of personal data handling are consented to" ;
                 rdfs:isDefinedBy "DPVCG" ;
                 sw:term_status "accepted" .


###  http://w3.org/ns/dpv#hasSector
dpv:hasSector rdf:type owl:ObjectProperty ;
              rdfs:domain dpv:Context ;
              rdfs:range dpv:Sector ;
              dct:created "2019-04-04"^^xsd:date ;
              dct:date-accepted "2019-04-05"^^xsd:date ;
              dct:description "Indicates the purpose is associated with activities in the indicated (Economic) Sector(s)"@en ;
              sw:term_status "accepted" .


###  http://w3.org/ns/dpv#hasTechnicalOrganisationalMeasure
dpv:hasTechnicalOrganisationalMeasure rdf:type owl:ObjectProperty ;
                                      rdfs:range dpv:TechnicalOrganisationalMeasure ;
                                      dct:created "2019-04-04"^^xsd:date ;
                                      dct:creator "Axel Polleres, Javier Ferenandez, Harshvardhan J. Pandit, Mark Lizar, Bud Bruegger" ;
                                      dct:date-accepted "2019-04-05"^^xsd:date ;
                                      dct:description "This property associates a technical/organisational measure with an instance of legal data handling or consent"@en ;
                                      rdfs:comment "We replicate all the properties except Legalbasis of personal data handling for consent, to declare what kinds of personal data handling are consented to" ;
                                      rdfs:isDefinedBy "DPVCG" ;
                                      sw:term_status "accepted" .


###  http://w3.org/ns/dpv#location
dpv:location rdf:type owl:ObjectProperty ;
             rdfs:domain dpv:StorageRestriction ;
             rdfs:range dpv:StorageLocation ;
             dct:created "2019-04-04"^^xsd:date ;
             dct:creator "Axel Polleres, Rob Brennan, Harshvardhan J. Pandit, Mark Lizar" ;
             dct:date-accepted "2019-04-05"^^xsd:date ;
             dct:description "Specifies location for storage of personal data"@en ;
             rdfs:isDefinedBy "DPVCG" ;
             sw:term_status "accepted" .


###  http://w3.org/ns/dpv#provisionBy
dpv:provisionBy rdf:type owl:ObjectProperty ;
                rdfs:domain dpv:Consent ;
                rdfs:range dpv:LegalEntity ;
                dct:created "2019-04-04"^^xsd:date ;
                dct:creator "Harshvardhan J. Pandit, Mark Lizar, Bud Bruegger" ;
                dct:date-accepted "2019-04-05"^^xsd:date ;
                dct:description "Specifies the entity that provisioned or provided consent"@en ;
                rdfs:comment "Normally this would be the dataSubject, but in some exceptional cases, the consent might be given on behalf by someone else, e.g. parents of minors." ;
                sw:term_status "accepted" .


###  http://w3.org/ns/dpv#provisionTime
dpv:provisionTime rdf:type owl:ObjectProperty ;
                  rdfs:domain dpv:Consent ;
                  rdfs:range time:Instant ;
                  dct:created "2019-04-04"^^xsd:date ;
                  dct:creator "Harshvardhan J. Pandit, Mark Lizar, Bud Bruegger" ;
                  dct:date-accepted "2019-04-05"^^xsd:date ;
                  dct:description "Specifies the instant in time when consent was given"@en ;
                  sw:term_status "accepted" .


###  http://w3.org/ns/dpv#storage
dpv:storage rdf:type owl:ObjectProperty ;
            rdfs:domain dpv:TechnicalOrganisationalMeasure ;
            rdfs:range dpv:StorageRestriction ;
            dct:created "2019-04-04"^^xsd:date ;
            dct:creator "Axel Polleres, Rob Brennan, Harshvardhan J. Pandit, Mark Lizar" ;
            dct:date-accepted "2019-04-05"^^xsd:date ;
            dct:description "Specifies restriction on the storage of personal data"@en ;
            rdfs:isDefinedBy "DPVCG" ;
            sw:term_status "accepted" .


###  http://w3.org/ns/dpv#withdrawalBy
dpv:withdrawalBy rdf:type owl:ObjectProperty ;
                 rdfs:domain dpv:Consent ;
                 rdfs:range dpv:LegalEntity ;
                 dct:created "2019-04-04"^^xsd:date ;
                 dct:creator "Harshvardhan J. Pandit, Mark Lizar, Bud Bruegger" ;
                 dct:date-accepted "2019-04-05"^^xsd:date ;
                 dct:description "Specifies the entity that withdrew consent"@en ;
                 rdfs:comment "Normally this would be the dataSubject, but in some exceptional cases, the consent might be withdraawn on behalf by someone else, e.g. parents of minors." ;
                 sw:term_status "accepted" .


###  http://w3.org/ns/dpv#withdrawalTime
dpv:withdrawalTime rdf:type owl:ObjectProperty ;
                   rdfs:domain dpv:Consent ;
                   rdfs:range time:Instant ;
                   dct:created "2019-04-04"^^xsd:date ;
                   dct:creator "Harshvardhan J. Pandit, Mark Lizar, Bud Bruegger" ;
                   dct:date-accepted "2019-04-05"^^xsd:date ;
                   dct:description "Specifies the instant in time when consent was withdrawn"@en ;
                   sw:term_status "accepted" .


#################################################################
#    Classes
#################################################################

###  http://w3.org/ns/dpv#A
dpv:A rdf:type owl:Class ;
      owl:disjointWith dpv:B .


###  http://w3.org/ns/dpv#AcademicResearch
dpv:AcademicResearch rdf:type owl:Class ;
                     rdfs:subClassOf dpv:ResearchAndDevelopment ;
                     dct:created "2018-12-10"^^xsd:date ;
                     dct:creator "Harshvardhan J. Pandit, Javier Fernandez, Axel Polleres, Elmar Kiesling, Fajar Ekaputra, Simon Steyskal" ;
                     dct:date-accepted "2019-04-05"^^xsd:date ;
                     dct:description "Research conducted in an academic context e.g. within universities"@en ;
                     rdfs:isDefinedBy <https://www.w3.org/community/dpvcg/wiki/Purposes_for_handling_Personal_Data#High-level_categories_.28to-be-discussed.29> ;
                     rdfs:seeAlso svpu:Education ;
                     sw:term_status "accepted" .


###  http://w3.org/ns/dpv#Accent
dpv:Accent rdf:type owl:Class ;
           rdfs:subClassOf dpv:Language ;
           dct:created "2019-04-04"^^xsd:date ;
           dct:creator "Elmar; Harshvardhan J. Pandit, Fajar" ;
           dct:date-accepted "2019-06-04"^^xsd:date ;
           dct:description "Information about an individual’s accent."@en ;
           rdfs:isDefinedBy <https://enterprivacy.com/wp-content/uploads/2018/09/Categories-of-Personal-Information.pdf> ;
           sw:term_status "accepted" .


###  http://w3.org/ns/dpv#AccessControl
dpv:AccessControl rdf:type owl:Class ;
                  rdfs:subClassOf dpv:Security ;
                  dct:created "2018-12-10"^^xsd:date ;
                  dct:creator "Harshvardhan J. Pandit, Javier Fernandez, Axel Polleres, Elmar Kiesling, Fajar Ekaputra, Simon Steyskal" ;
                  dct:date-accepted "2019-04-05"^^xsd:date ;
                  dct:description "To conduct or enforce access control"@en ;
                  rdfs:isDefinedBy <https://www.w3.org/community/dpvcg/wiki/Purposes_for_handling_Personal_Data#High-level_categories_.28to-be-discussed.29> ;
                  rdfs:seeAlso svpu:Login ;
                  sw:term_status "accepted" .


###  http://w3.org/ns/dpv#AccessControlMethod
dpv:AccessControlMethod rdf:type owl:Class ;
                        rdfs:subClassOf dpv:TechnicalMeasure ;
                        dct:created "2019-04-04"^^xsd:date ;
                        dct:creator "Axel Polleres, Rob Brennan, Harshvardhan J. Pandit, Mark Lizar" ;
                        dct:date-accepted "2019-04-05"^^xsd:date ;
                        dct:description "methods which restrict access to a place or resource"@en ;
                        rdfs:isDefinedBy "DPVCG" ;
                        sw:term_status "accepted" .


###  http://w3.org/ns/dpv#AccountIdentifier
dpv:AccountIdentifier rdf:type owl:Class ;
                      rdfs:subClassOf dpv:FinancialAccount ;
                      dct:created "2019-04-04"^^xsd:date ;
                      dct:creator "Elmar; Harshvardhan J. Pandit, Fajar" ;
                      dct:date-accepted "2019-06-04"^^xsd:date ;
                      dct:description "Information about an individual's financial account identifier."@en ;
                      rdfs:isDefinedBy <https://enterprivacy.com/wp-content/uploads/2018/09/Categories-of-Personal-Information.pdf> ;
                      sw:term_status "accepted" .


###  http://w3.org/ns/dpv#Acquantaince
dpv:Acquantaince rdf:type owl:Class ;
                 rdfs:subClassOf dpv:SocialNetwork ;
                 dct:created "2019-04-04"^^xsd:date ;
                 dct:creator "Elmar; Harshvardhan J. Pandit, Fajar" ;
                 dct:date-accepted "2019-06-04"^^xsd:date ;
                 dct:description "Information about acquaintainces in a social network."@en ;
                 rdfs:isDefinedBy <https://enterprivacy.com/wp-content/uploads/2018/09/Categories-of-Personal-Information.pdf> ;
                 sw:term_status "accepted" .


###  http://w3.org/ns/dpv#Acquire
dpv:Acquire rdf:type owl:Class ;
            rdfs:subClassOf dpv:Obtain ;
            dct:created "2019-04-04"^^xsd:date ;
            dct:date-accepted "2019-05-07"^^xsd:date ;
            dct:description "to come into possession or control of the data"@en ;
            rdfs:isDefinedBy "DPVCG" ;
            sw:term_status "accepted" .


###  http://w3.org/ns/dpv#Adapt
dpv:Adapt rdf:type owl:Class ;
          rdfs:subClassOf dpv:Transform ;
          dct:created "2019-04-04"^^xsd:date ;
          dct:date-accepted "2019-05-07"^^xsd:date ;
          dct:description "to modify the data, often rewritten into a new form for a new use"@en ;
          rdfs:isDefinedBy <https://eur-lex.europa.eu/eli/reg/2016/679/art_4/par_2/oj> ;
          sw:term_status "accepted" .


###  http://w3.org/ns/dpv#Age
dpv:Age rdf:type owl:Class ;
        rdfs:subClassOf dpv:PhysicalCharacteristic ;
        dct:created "2019-04-04"^^xsd:date ;
        dct:creator "Elmar; Harshvardhan J. Pandit, Fajar" ;
        dct:date-accepted "2019-06-04"^^xsd:date ;
        dct:description "Information about an individual's age"@en ;
        rdfs:isDefinedBy <https://enterprivacy.com/wp-content/uploads/2018/09/Categories-of-Personal-Information.pdf> ;
        sw:term_status "accepted" .


###  http://w3.org/ns/dpv#Align
dpv:Align rdf:type owl:Class ;
          rdfs:subClassOf dpv:Transform ;
          dct:created "2019-04-04"^^xsd:date ;
          dct:date-accepted "2019-05-07"^^xsd:date ;
          dct:description "to adjust the data to be in relation to another data"@en ;
          rdfs:isDefinedBy <https://eur-lex.europa.eu/eli/reg/2016/679/art_4/par_2/oj> ;
          sw:term_status "accepted" .


###  http://w3.org/ns/dpv#Alter
dpv:Alter rdf:type owl:Class ;
          rdfs:subClassOf dpv:Transform ;
          dct:created "2019-04-04"^^xsd:date ;
          dct:date-accepted "2019-05-07"^^xsd:date ;
          dct:description "to change the data withouth changing it into something else"@en ;
          rdfs:isDefinedBy <https://eur-lex.europa.eu/eli/reg/2016/679/art_4/par_2/oj> ;
          sw:term_status "accepted" .


###  http://w3.org/ns/dpv#Analyse
dpv:Analyse rdf:type owl:Class ;
            rdfs:subClassOf dpv:Use ;
            dct:created "2019-04-04"^^xsd:date ;
            dct:date-accepted "2019-05-07"^^xsd:date ;
            dct:description "to study or examine the data in detail"@en ;
            rdfs:isDefinedBy <https://www.specialprivacy.eu/vocabs/processing> ;
            rdfs:seeAlso svpr:Analyse ;
            sw:term_status "accepted" .


###  http://w3.org/ns/dpv#Anonymise
dpv:Anonymise rdf:type owl:Class ;
              rdfs:subClassOf dpv:Transform ;
              dct:created "2019-04-04"^^xsd:date ;
              dct:date-accepted "2019-05-07"^^xsd:date ;
              dct:description "to irreversibly alter personal data in such a way that a unique data subject can no longer be identified directly or indirectly or in combination with other data"@en ;
              rdfs:isDefinedBy <https://www.specialprivacy.eu/vocabs/processing> ;
              rdfs:seeAlso svpr:Anonymize ;
              sw:term_status "accepted" .


###  http://w3.org/ns/dpv#Anonymization
dpv:Anonymization rdf:type owl:Class ;
                  rdfs:subClassOf dpv:PseudoAnonymization ;
                  dct:created "2019-04-04"^^xsd:date ;
                  dct:creator "Axel Polleres, Rob Brennan, Harshvardhan J. Pandit, Mark Lizar" ;
                  dct:date-accepted "2019-04-05"^^xsd:date ;
                  dct:description "process by which personal data is irreversibly altered in such a way that a data subject can no longer be identified directly or indirectly, either by the data controller alone or in collaboration with any other party"@en ;
                  rdfs:isDefinedBy "DPVCG" ;
                  sw:term_status "accepted" .


###  http://w3.org/ns/dpv#ApartmentOwned
dpv:ApartmentOwned rdf:type owl:Class ;
                   rdfs:subClassOf dpv:HouseOwned ;
                   dct:created "2019-04-04"^^xsd:date ;
                   dct:creator "Elmar; Harshvardhan J. Pandit, Fajar" ;
                   dct:date-accepted "2019-06-04"^^xsd:date ;
                   dct:description "Information on the apartement(s) owned by an individual."@en ;
                   rdfs:isDefinedBy <https://enterprivacy.com/wp-content/uploads/2018/09/Categories-of-Personal-Information.pdf> ;
                   sw:term_status "accepted" .


###  http://w3.org/ns/dpv#Association
dpv:Association rdf:type owl:Class ;
                rdfs:subClassOf dpv:SocialNetwork ;
                dct:created "2019-04-04"^^xsd:date ;
                dct:creator "Elmar; Harshvardhan J. Pandit, Fajar" ;
                dct:date-accepted "2019-06-04"^^xsd:date ;
                dct:description "Information about associations in a social network with other individuals, groups, or entities e.g. friend of a friend"@en ;
                rdfs:isDefinedBy <https://enterprivacy.com/wp-content/uploads/2018/09/Categories-of-Personal-Information.pdf> ;
                sw:term_status "accepted" .


###  http://w3.org/ns/dpv#Attitude
dpv:Attitude rdf:type owl:Class ;
             rdfs:subClassOf dpv:Behavioral ;
             dct:created "2019-04-04"^^xsd:date ;
             dct:creator "Elmar; Harshvardhan J. Pandit, Fajar" ;
             dct:date-accepted "2019-06-04"^^xsd:date ;
             dct:description "Information that relates to an individual's attitude."@en ;
             rdfs:isDefinedBy <https://enterprivacy.com/wp-content/uploads/2018/09/Categories-of-Personal-Information.pdf> ;
             sw:term_status "accepted" .


###  http://w3.org/ns/dpv#Authenticating
dpv:Authenticating rdf:type owl:Class ;
                   rdfs:subClassOf dpv:Internal ;
                   dct:created "2019-04-04"^^xsd:date ;
                   dct:creator "Elmar; Harshvardhan J. Pandit, Fajar" ;
                   dct:date-accepted "2019-06-04"^^xsd:date ;
                   dct:description "Information used to authenticate an individual with something they know"@en ;
                   rdfs:isDefinedBy <https://enterprivacy.com/wp-content/uploads/2018/09/Categories-of-Personal-Information.pdf> ;
                   sw:term_status "accepted" .


###  http://w3.org/ns/dpv#AuthenticationProtocols
dpv:AuthenticationProtocols rdf:type owl:Class ;
                            rdfs:subClassOf dpv:TechnicalMeasure ;
                            dct:created "2019-04-04"^^xsd:date ;
                            dct:creator "Axel Polleres, Rob Brennan, Harshvardhan J. Pandit, Mark Lizar" ;
                            dct:date-accepted "2019-04-05"^^xsd:date ;
                            dct:description "protocols involving validation of identity i.e. authentication of a person or information"@en ;
                            rdfs:isDefinedBy "DPVCG" ;
                            sw:term_status "accepted" .


###  http://w3.org/ns/dpv#AuthorisationProcedure
dpv:AuthorisationProcedure rdf:type owl:Class ;
                           rdfs:subClassOf dpv:OrganisationalMeasure ;
                           dct:created "2019-04-04"^^xsd:date ;
                           dct:creator "Axel Polleres, Rob Brennan, Harshvardhan J. Pandit, Mark Lizar" ;
                           dct:date-accepted "2019-04-05"^^xsd:date ;
                           dct:description "Specifies procedures for determining permission or authority"@en ;
                           rdfs:isDefinedBy "DPVCG" ;
                           sw:term_status "accepted" .


###  http://w3.org/ns/dpv#B
dpv:B rdf:type owl:Class .


###  http://w3.org/ns/dpv#BankAccount
dpv:BankAccount rdf:type owl:Class ;
                rdfs:subClassOf dpv:FinancialAccount ;
                dct:created "2019-04-04"^^xsd:date ;
                dct:creator "Elmar; Harshvardhan J. Pandit, Fajar" ;
                dct:date-accepted "2019-06-04"^^xsd:date ;
                dct:description "Information related to an individual's bank account."@en ;
                rdfs:isDefinedBy <https://enterprivacy.com/wp-content/uploads/2018/09/Categories-of-Personal-Information.pdf> ;
                sw:term_status "accepted" .


###  http://w3.org/ns/dpv#Behavioral
dpv:Behavioral rdf:type owl:Class ;
               rdfs:subClassOf dpv:External ;
               dct:created "2019-04-04"^^xsd:date ;
               dct:creator "Elmar; Harshvardhan J. Pandit, Fajar" ;
               dct:date-accepted "2019-06-04"^^xsd:date ;
               dct:description "Information that describes an individual’s behavior or activity, on-line or off"@en ;
               rdfs:isDefinedBy <https://enterprivacy.com/wp-content/uploads/2018/09/Categories-of-Personal-Information.pdf> ;
               rdfs:seeAlso svd:Activity ;
               sw:term_status "accepted" .


###  http://w3.org/ns/dpv#Beneficiary
dpv:Beneficiary rdf:type owl:Class ;
                dct:created "2019-05-23"^^xsd:date ;
                dct:description "self.DataSubject, self.DataController, society ? ( --- under consideration ---)"@en ;
                sw:term_status "proposed" .


###  http://w3.org/ns/dpv#Biometric
dpv:Biometric rdf:type owl:Class ;
              rdfs:subClassOf dpv:Identifying ,
                              dpv:SpecialCategoryPersonalData ;
              dct:created "2019-04-04"^^xsd:date ;
              dct:creator "Elmar; Harshvardhan J. Pandit, Fajar" ;
              dct:date-accepted "2019-06-04"^^xsd:date ;
              dct:description "Biometric information on an individual."@en ;
              rdfs:isDefinedBy <https://enterprivacy.com/wp-content/uploads/2018/09/Categories-of-Personal-Information.pdf> ;
              sw:term_status "accepted" .


###  http://w3.org/ns/dpv#BloodType
dpv:BloodType rdf:type owl:Class ;
              rdfs:subClassOf dpv:MedicalHealth ;
              dct:created "2019-04-04"^^xsd:date ;
              dct:creator "Elmar; Harshvardhan J. Pandit, Fajar" ;
              dct:date-accepted "2019-06-04"^^xsd:date ;
              dct:description "Information about an individual's blood type."@en ;
              rdfs:isDefinedBy <https://enterprivacy.com/wp-content/uploads/2018/09/Categories-of-Personal-Information.pdf> ;
              sw:term_status "accepted" .


###  http://w3.org/ns/dpv#BrowserFingerprint
dpv:BrowserFingerprint rdf:type owl:Class ;
                       rdfs:subClassOf dpv:DeviceBased ;
                       dct:created "2019-04-04"^^xsd:date ;
                       dct:creator "Elmar; Harshvardhan J. Pandit, Fajar" ;
                       dct:date-accepted "2019-06-04"^^xsd:date ;
                       dct:description "Information that characterizes the browser used by an individual, which in turn can be used to uniquely identify a user."@en ;
                       rdfs:isDefinedBy <https://enterprivacy.com/wp-content/uploads/2018/09/Categories-of-Personal-Information.pdf> ;
                       sw:term_status "accepted" .


###  http://w3.org/ns/dpv#BrowsingBehavior
dpv:BrowsingBehavior rdf:type owl:Class ;
                     rdfs:subClassOf dpv:Behavioral ;
                     dct:created "2019-04-04"^^xsd:date ;
                     dct:creator "Elmar; Harshvardhan J. Pandit, Fajar" ;
                     dct:date-accepted "2019-06-04"^^xsd:date ;
                     dct:description "Information that relates to an individual's browsing behaviour."@en ;
                     rdfs:isDefinedBy <https://enterprivacy.com/wp-content/uploads/2018/09/Categories-of-Personal-Information.pdf> ;
                     rdfs:seeAlso svd:OnlineActivity ;
                     sw:term_status "accepted" .


###  http://w3.org/ns/dpv#CallLog
dpv:CallLog rdf:type owl:Class ;
            rdfs:subClassOf dpv:Behavioral ;
            dct:created "2019-04-04"^^xsd:date ;
            dct:creator "Elmar; Harshvardhan J. Pandit, Fajar" ;
            dct:date-accepted "2019-06-04"^^xsd:date ;
            dct:description "Information on the calls that an individual has made."@en ;
            rdfs:isDefinedBy <https://enterprivacy.com/wp-content/uploads/2018/09/Categories-of-Personal-Information.pdf> ;
            sw:term_status "accepted" .


###  http://w3.org/ns/dpv#CarOwned
dpv:CarOwned rdf:type owl:Class ;
             rdfs:subClassOf dpv:Ownership ;
             dct:created "2019-04-04"^^xsd:date ;
             dct:creator "Elmar; Harshvardhan J. Pandit, Fajar" ;
             dct:date-accepted "2019-06-04"^^xsd:date ;
             dct:description "Information about cars owned by an individual."@en ;
             rdfs:isDefinedBy <https://enterprivacy.com/wp-content/uploads/2018/09/Categories-of-Personal-Information.pdf> ;
             sw:term_status "accepted" .


###  http://w3.org/ns/dpv#Certification
dpv:Certification rdf:type owl:Class ;
                  rdfs:subClassOf dpv:CertificationSeal ,
                                  dpv:Professional ;
                  dct:created "2019-04-04"^^xsd:date ;
                  dct:creator "Axel Polleres, Rob Brennan, Harshvardhan J. Pandit, Mark Lizar" ,
                              "Elmar; Harshvardhan J. Pandit, Fajar" ;
                  dct:date-accepted "2019-04-05"^^xsd:date ,
                                    "2019-06-04"^^xsd:date ;
                  dct:description "Information about professional certifications associated with an individual"@en ,
                                  "certification mechanisms, seals, and marks for the purpose of demonstrating compliance"@en ;
                  rdfs:isDefinedBy <https://enterprivacy.com/wp-content/uploads/2018/09/Categories-of-Personal-Information.pdf> ,
                                   "DPVCG" ;
                  sw:term_status "accepted" .


###  http://w3.org/ns/dpv#CertificationSeal
dpv:CertificationSeal rdf:type owl:Class ;
                      rdfs:subClassOf dpv:OrganisationalMeasure ;
                      dct:created "2019-04-04"^^xsd:date ;
                      dct:creator "Axel Polleres, Rob Brennan, Harshvardhan J. Pandit, Mark Lizar" ;
                      dct:date-accepted "2019-04-05"^^xsd:date ;
                      dct:description "Category of certifications, seals, and marks indicating compliance to regulations or practices"@en ;
                      rdfs:isDefinedBy "DPVCG" ;
                      sw:term_status "accepted" .


###  http://w3.org/ns/dpv#Character
dpv:Character rdf:type owl:Class ;
              rdfs:subClassOf dpv:PublicLife ;
              dct:created "2019-04-04"^^xsd:date ;
              dct:creator "Elmar; Harshvardhan J. Pandit, Fajar" ;
              dct:date-accepted "2019-06-04"^^xsd:date ;
              dct:description "Information about an individual's character in the public sphere"@en ;
              rdfs:isDefinedBy <https://enterprivacy.com/wp-content/uploads/2018/09/Categories-of-Personal-Information.pdf> ;
              sw:term_status "accepted" .


###  http://w3.org/ns/dpv#Child
dpv:Child rdf:type owl:Class ;
          rdfs:subClassOf dpv:DataSubject ;
          dct:created "2019-06-06"^^xsd:date ;
          dct:creator "Harshvardhan J. Pandit" ;
          dct:description "A 'child' is a natural legal person who is below a certain legal age depending on the legal jurisdiction."@en ;
          rdfs:comment "A 'child' is distinct from a 'minor'. For example, the legal age for a 'minor' in most countries is 18, whereas a 'child' can be a minor below the age of 14." ;
          sw:term_status "proposed" .


###  http://w3.org/ns/dpv#CodeOfConduct
dpv:CodeOfConduct rdf:type owl:Class ;
                  rdfs:subClassOf dpv:GuidelinesPrinciple ;
                  dct:created "2019-04-04"^^xsd:date ;
                  dct:creator "Axel Polleres, Rob Brennan, Harshvardhan J. Pandit, Mark Lizar" ;
                  dct:date-accepted "2019-04-05"^^xsd:date ;
                  dct:description "A set of rules or procedures outlining the norms and practices for conducting activities"@en ;
                  rdfs:isDefinedBy "DPVCG" ;
                  sw:term_status "accepted" .


###  http://w3.org/ns/dpv#Collect
dpv:Collect rdf:type owl:Class ;
            rdfs:subClassOf dpv:Obtain ;
            dct:created "2019-04-04"^^xsd:date ;
            dct:date-accepted "2019-05-07"^^xsd:date ;
            dct:description "to gather data from someone"@en ;
            rdfs:isDefinedBy <https://eur-lex.europa.eu/eli/reg/2016/679/art_4/par_2/oj> ,
                             "DPVCG" ;
            rdfs:seeAlso svpr:Collect ;
            sw:term_status "accepted" .


###  http://w3.org/ns/dpv#Combine
dpv:Combine rdf:type owl:Class ;
            rdfs:subClassOf dpv:Transform ;
            dct:created "2019-04-04"^^xsd:date ;
            dct:date-accepted "2019-05-07"^^xsd:date ;
            dct:description "to join or merge data"@en ;
            rdfs:isDefinedBy <https://eur-lex.europa.eu/eli/reg/2016/679/art_4/par_2/oj> ,
                             "DPVCG" ;
            rdfs:seeAlso svpr:Aggregate ;
            sw:term_status "accepted" .


###  http://w3.org/ns/dpv#CommercialInterest
dpv:CommercialInterest rdf:type owl:Class ;
                       rdfs:subClassOf dpv:Purpose ;
                       dct:created "2018-12-10"^^xsd:date ;
                       dct:creator "Harshvardhan J. Pandit, Javier Fernandez, Axel Polleres, Elmar Kiesling, Fajar Ekaputra, Simon Steyskal" ;
                       dct:date-accepted "2019-04-05"^^xsd:date ;
                       dct:description "For purposes of commercial activities i.e. of profit or benefit to the Controller"@en ;
                       rdfs:isDefinedBy <https://www.w3.org/community/dpvcg/wiki/Purposes_for_handling_Personal_Data#High-level_categories_.28to-be-discussed.29> ;
                       sw:term_status "accepted" .


###  http://w3.org/ns/dpv#CommercialResearch
dpv:CommercialResearch rdf:type owl:Class ;
                       rdfs:subClassOf dpv:ResearchAndDevelopment ;
                       dct:created "2018-12-10"^^xsd:date ;
                       dct:creator "Harshvardhan J. Pandit, Javier Fernandez, Axel Polleres, Elmar Kiesling, Fajar Ekaputra, Simon Steyskal" ;
                       dct:date-accepted "2019-04-05"^^xsd:date ;
                       dct:description "Research conducted in a commercial setting e.g. in a company"@en ;
                       rdfs:isDefinedBy <https://www.w3.org/community/dpvcg/wiki/Purposes_for_handling_Personal_Data#High-level_categories_.28to-be-discussed.29> ;
                       rdfs:seeAlso svpu:Develop ;
                       sw:term_status "accepted" .


###  http://w3.org/ns/dpv#Communication
dpv:Communication rdf:type owl:Class ;
                  rdfs:subClassOf dpv:Social ;
                  dct:created "2019-04-04"^^xsd:date ;
                  dct:creator "Elmar; Harshvardhan J. Pandit, Fajar" ;
                  dct:date-accepted "2019-06-04"^^xsd:date ;
                  dct:description "Information communicated from or to an individual"@en ;
                  rdfs:isDefinedBy <https://enterprivacy.com/wp-content/uploads/2018/09/Categories-of-Personal-Information.pdf> ;
                  sw:term_status "accepted" .


###  http://w3.org/ns/dpv#CommunicationsMetadata
dpv:CommunicationsMetadata rdf:type owl:Class ;
                           rdfs:subClassOf dpv:PublicLife ;
                           dct:created "2019-04-04"^^xsd:date ;
                           dct:creator "Elmar; Harshvardhan J. Pandit, Fajar" ;
                           dct:date-accepted "2019-06-04"^^xsd:date ;
                           dct:description "Information about communication metadata in the public sphere"@en ;
                           rdfs:isDefinedBy <https://enterprivacy.com/wp-content/uploads/2018/09/Categories-of-Personal-Information.pdf> ;
                           rdfs:seeAlso svd:Interactive ;
                           sw:term_status "accepted" .


###  http://w3.org/ns/dpv#Connection
dpv:Connection rdf:type owl:Class ;
               rdfs:subClassOf dpv:SocialNetwork ;
               dct:created "2019-04-04"^^xsd:date ;
               dct:creator "Elmar; Harshvardhan J. Pandit, Fajar" ;
               dct:date-accepted "2019-06-04"^^xsd:date ;
               dct:description "Information about and including connections of an individual in a social network"@en ;
               rdfs:isDefinedBy <https://enterprivacy.com/wp-content/uploads/2018/09/Categories-of-Personal-Information.pdf> ;
               sw:term_status "accepted" .


###  http://w3.org/ns/dpv#Consent
dpv:Consent rdf:type owl:Class ;
            dct:created "2019-04-04"^^xsd:date ;
            dct:creator "Harshvardhan J. Pandit, Mark Lizar, Bud Bruegger" ;
            dct:date-accepted "2019-04-05"^^xsd:date ;
            dct:description "Consent as defined by Article 4(11) of the GDPR"@en ;
            rdfs:isDefinedBy <https://eur-lex.europa.eu/eli/reg/2016/679/art_4/par_11/oj> ;
            sw:term_status "accepted" .


###  http://w3.org/ns/dpv#Consult
dpv:Consult rdf:type owl:Class ;
            rdfs:subClassOf dpv:Use ;
            dct:created "2019-04-04"^^xsd:date ;
            dct:date-accepted "2019-05-07"^^xsd:date ;
            dct:description "to consult or query data"@en ;
            rdfs:isDefinedBy <https://eur-lex.europa.eu/eli/reg/2016/679/art_4/par_2/oj> ,
                             "DPVCG" ;
            rdfs:seeAlso svpr:Query ;
            sw:term_status "accepted" .


###  http://w3.org/ns/dpv#Contact
dpv:Contact rdf:type owl:Class ;
            rdfs:subClassOf dpv:Tracking ;
            dct:created "2019-04-04"^^xsd:date ;
            dct:creator "Elmar; Harshvardhan J. Pandit, Fajar" ;
            dct:date-accepted "2019-06-04"^^xsd:date ;
            dct:description "Information that can be used for contacting an individual e.g. email address or phone number"@en ;
            rdfs:isDefinedBy <https://enterprivacy.com/wp-content/uploads/2018/09/Categories-of-Personal-Information.pdf> ;
            rdfs:seeAlso svd:Physical ;
            sw:term_status "accepted" .


###  http://w3.org/ns/dpv#Context
dpv:Context rdf:type owl:Class ;
            dct:created "2019-04-04"^^xsd:date ;
            dct:date-accepted "2019-04-05"^^xsd:date ;
            dct:description "Used to scope the purpose, e.g. restriction to a certain business sector"@en ;
            sw:term_status "accepted" .


###  http://w3.org/ns/dpv#Contract
dpv:Contract rdf:type owl:Class ;
             rdfs:subClassOf dpv:LegalAgreement ;
             dct:created "2019-04-04"^^xsd:date ;
             dct:creator "Axel Polleres, Rob Brennan, Harshvardhan J. Pandit, Mark Lizar" ;
             dct:date-accepted "2019-04-05"^^xsd:date ;
             dct:description "Contractual terms governing data handling within the data controller"@en ;
             rdfs:isDefinedBy "DPVCG" ;
             sw:term_status "accepted" .


###  http://w3.org/ns/dpv#Copy
dpv:Copy rdf:type owl:Class ;
         rdfs:subClassOf dpv:Processing ;
         dct:created "2019-04-04"^^xsd:date ;
         dct:date-accepted "2019-05-07"^^xsd:date ;
         dct:description "to produce an exact reprodution of the data"@en ;
         rdfs:isDefinedBy <https://www.specialprivacy.eu/vocabs/processing> ;
         rdfs:seeAlso svpr:Copy ;
         sw:term_status "accepted" .


###  http://w3.org/ns/dpv#Country
dpv:Country rdf:type owl:Class ;
            rdfs:subClassOf dpv:Location ;
            dct:created "2019-04-04"^^xsd:date ;
            dct:creator "Elmar; Harshvardhan J. Pandit, Fajar" ;
            dct:date-accepted "2019-06-04"^^xsd:date ;
            dct:description "Information about an individual’s country e.g. residence, travel."@en ;
            rdfs:isDefinedBy <https://enterprivacy.com/wp-content/uploads/2018/09/Categories-of-Personal-Information.pdf> ;
            sw:term_status "accepted" .


###  http://w3.org/ns/dpv#CreateEventRecommendations
dpv:CreateEventRecommendations rdf:type owl:Class ;
                               rdfs:subClassOf dpv:CreatePersonalizedRecommendations ;
                               dct:created "2019-11-25"^^xsd:date ;
                               dct:creator "Harshvardhan J. Pandit, Rudy Jacob" ;
                               dct:description "Create and provide personalised recommendations for events to the individual."@en ;
                               sw:term_status "proposed" .


###  http://w3.org/ns/dpv#CreatePersonalizedRecommendations
dpv:CreatePersonalizedRecommendations rdf:type owl:Class ;
                                      rdfs:subClassOf dpv:ServicePersonalization ;
                                      dct:created "2019-11-25"^^xsd:date ;
                                      dct:creator "Harshvardhan J. Pandit, Rudy Jacob" ;
                                      dct:description "Create and provide personalised recommendations to the individual."@en ;
                                      sw:term_status "proposed" .


###  http://w3.org/ns/dpv#CreateProductRecommendations
dpv:CreateProductRecommendations rdf:type owl:Class ;
                                 rdfs:subClassOf dpv:CreatePersonalizedRecommendations ;
                                 dct:created "2018-12-10"^^xsd:date ;
                                 dct:creator "Harshvardhan J. Pandit, Javier Fernandez, Axel Polleres, Elmar Kiesling, Fajar Ekaputra, Simon Steyskal" ;
                                 dct:date-accepted "2019-04-05"^^xsd:date ;
                                 dct:description "To create product recommendations e.g. suggest similar products"@en ;
                                 dct:modified "2019-11-25"^^xsd:date ;
                                 rdfs:isDefinedBy <https://www.w3.org/community/dpvcg/wiki/Purposes_for_handling_Personal_Data#High-level_categories_.28to-be-discussed.29> ;
                                 rdfs:seeAlso svpu:Marketing ;
                                 sw:term_status "accepted" .


###  http://w3.org/ns/dpv#Credit
dpv:Credit rdf:type owl:Class ;
           rdfs:subClassOf dpv:Financial ,
                           dpv:Transactional ;
           dct:created "2019-04-04"^^xsd:date ;
           dct:creator "Elmar; Harshvardhan J. Pandit, Fajar" ;
           dct:date-accepted "2019-06-04"^^xsd:date ;
           dct:description "Information about an individual’s reputation with regards to money"@en ;
           rdfs:isDefinedBy <https://enterprivacy.com/wp-content/uploads/2018/09/Categories-of-Personal-Information.pdf> ;
           sw:term_status "accepted" .


###  http://w3.org/ns/dpv#CreditCapacity
dpv:CreditCapacity rdf:type owl:Class ;
                   rdfs:subClassOf dpv:Credit ;
                   dct:created "2019-04-04"^^xsd:date ;
                   dct:creator "Elmar; Harshvardhan J. Pandit, Fajar" ;
                   dct:date-accepted "2019-06-04"^^xsd:date ;
                   dct:description "Information relating to an individual's credit capacity."@en ;
                   rdfs:isDefinedBy <https://enterprivacy.com/wp-content/uploads/2018/09/Categories-of-Personal-Information.pdf> ;
                   sw:term_status "accepted" .


###  http://w3.org/ns/dpv#CreditCardNumber
dpv:CreditCardNumber rdf:type owl:Class ;
                     rdfs:subClassOf dpv:AccountIdentifier ;
                     dct:created "2019-04-04"^^xsd:date ;
                     dct:creator "Elmar; Harshvardhan J. Pandit, Fajar" ;
                     dct:date-accepted "2019-06-04"^^xsd:date ;
                     dct:description "Information about an individual's credit card number"@en ;
                     rdfs:isDefinedBy <https://enterprivacy.com/wp-content/uploads/2018/09/Categories-of-Personal-Information.pdf> ;
                     sw:term_status "accepted" .


###  http://w3.org/ns/dpv#CreditRecord
dpv:CreditRecord rdf:type owl:Class ;
                 rdfs:subClassOf dpv:Credit ;
                 dct:created "2019-04-04"^^xsd:date ;
                 dct:creator "Elmar; Harshvardhan J. Pandit, Fajar" ;
                 dct:date-accepted "2019-06-04"^^xsd:date ;
                 dct:description "Information relating to an individual's credit record."@en ;
                 rdfs:isDefinedBy <https://enterprivacy.com/wp-content/uploads/2018/09/Categories-of-Personal-Information.pdf> ;
                 sw:term_status "accepted" .


###  http://w3.org/ns/dpv#CreditScore
dpv:CreditScore rdf:type owl:Class ;
                rdfs:subClassOf dpv:CreditWorthiness ;
                dct:created "2019-04-04"^^xsd:date ;
                dct:creator "Elmar; Harshvardhan J. Pandit, Fajar" ;
                dct:date-accepted "2019-06-04"^^xsd:date ;
                dct:description "Information relating to an individual's credit score."@en ;
                rdfs:isDefinedBy <https://enterprivacy.com/wp-content/uploads/2018/09/Categories-of-Personal-Information.pdf> ;
                sw:term_status "accepted" .


###  http://w3.org/ns/dpv#CreditStanding
dpv:CreditStanding rdf:type owl:Class ;
                   rdfs:subClassOf dpv:Credit ;
                   dct:created "2019-04-04"^^xsd:date ;
                   dct:creator "Elmar; Harshvardhan J. Pandit, Fajar" ;
                   dct:date-accepted "2019-06-04"^^xsd:date ;
                   dct:description "Information relating to an individual's credit standing."@en ;
                   rdfs:isDefinedBy <https://enterprivacy.com/wp-content/uploads/2018/09/Categories-of-Personal-Information.pdf> ;
                   sw:term_status "accepted" .


###  http://w3.org/ns/dpv#CreditWorthiness
dpv:CreditWorthiness rdf:type owl:Class ;
                     rdfs:subClassOf dpv:Credit ;
                     dct:created "2019-04-04"^^xsd:date ;
                     dct:creator "Elmar; Harshvardhan J. Pandit, Fajar" ;
                     dct:date-accepted "2019-06-04"^^xsd:date ;
                     dct:description "Information relating to an individual's credit worthiness."@en ;
                     rdfs:isDefinedBy <https://enterprivacy.com/wp-content/uploads/2018/09/Categories-of-Personal-Information.pdf> ;
                     sw:term_status "accepted" .


###  http://w3.org/ns/dpv#Criminal
dpv:Criminal rdf:type owl:Class ;
             rdfs:subClassOf dpv:Social ;
             dct:created "2019-04-04"^^xsd:date ;
             dct:creator "Elmar; Harshvardhan J. Pandit, Fajar" ;
             dct:date-accepted "2019-06-04"^^xsd:date ;
             dct:description "Information about an individual’s criminal activity e.g. criminal convictions or jail time"@en ;
             rdfs:isDefinedBy <https://enterprivacy.com/wp-content/uploads/2018/09/Categories-of-Personal-Information.pdf> ;
             rdfs:seeAlso svd:Judicial ;
             sw:term_status "accepted" .


###  http://w3.org/ns/dpv#CriminalCharge
dpv:CriminalCharge rdf:type owl:Class ;
                   rdfs:subClassOf dpv:Criminal ;
                   dct:created "2019-04-04"^^xsd:date ;
                   dct:creator "Elmar; Harshvardhan J. Pandit, Fajar" ;
                   dct:date-accepted "2019-06-04"^^xsd:date ;
                   dct:description "Information on an individual's criminal charges."@en ;
                   rdfs:isDefinedBy <https://enterprivacy.com/wp-content/uploads/2018/09/Categories-of-Personal-Information.pdf> ;
                   sw:term_status "accepted" .


###  http://w3.org/ns/dpv#CriminalConviction
dpv:CriminalConviction rdf:type owl:Class ;
                       rdfs:subClassOf dpv:Criminal ;
                       dct:created "2019-04-04"^^xsd:date ;
                       dct:creator "Elmar; Harshvardhan J. Pandit, Fajar" ;
                       dct:date-accepted "2019-06-04"^^xsd:date ;
                       dct:description "Information on an individual's criminal convictions."@en ;
                       rdfs:isDefinedBy <https://enterprivacy.com/wp-content/uploads/2018/09/Categories-of-Personal-Information.pdf> ;
                       sw:term_status "accepted" .


###  http://w3.org/ns/dpv#CriminalPardon
dpv:CriminalPardon rdf:type owl:Class ;
                   rdfs:subClassOf dpv:Criminal ;
                   dct:created "2019-04-04"^^xsd:date ;
                   dct:creator "Elmar; Harshvardhan J. Pandit, Fajar" ;
                   dct:date-accepted "2019-06-04"^^xsd:date ;
                   dct:description "Information on an individual's criminal pardons."@en ;
                   rdfs:isDefinedBy <https://enterprivacy.com/wp-content/uploads/2018/09/Categories-of-Personal-Information.pdf> ;
                   sw:term_status "accepted" .


###  http://w3.org/ns/dpv#CustomerCare
dpv:CustomerCare rdf:type owl:Class ;
                 rdfs:subClassOf dpv:ServiceProvision ;
                 dct:created "2018-12-10"^^xsd:date ;
                 dct:creator "Harshvardhan J. Pandit, Javier Fernandez, Axel Polleres, Elmar Kiesling, Fajar Ekaputra, Simon Steyskal" ;
                 dct:date-accepted "2019-04-05"^^xsd:date ;
                 dct:description "Processes related to providing assistance for customer satisfaction"@en ;
                 rdfs:isDefinedBy <https://www.w3.org/community/dpvcg/wiki/Purposes_for_handling_Personal_Data#High-level_categories_.28to-be-discussed.29> ;
                 rdfs:seeAlso svpu:Feedback ;
                 sw:term_status "accepted" .


###  http://w3.org/ns/dpv#DNACode
dpv:DNACode rdf:type owl:Class ;
            rdfs:subClassOf dpv:MedicalHealth ;
            dct:created "2019-04-04"^^xsd:date ;
            dct:creator "Elmar; Harshvardhan J. Pandit, Fajar" ;
            dct:date-accepted "2019-06-04"^^xsd:date ;
            dct:description "Information about an individual's DNA."@en ;
            rdfs:isDefinedBy <https://enterprivacy.com/wp-content/uploads/2018/09/Categories-of-Personal-Information.pdf> ;
            sw:term_status "accepted" .


###  http://w3.org/ns/dpv#DataController
dpv:DataController rdf:type owl:Class ;
                   dct:created "2019-04-04"^^xsd:date ;
                   dct:creator "Axel Polleres, Javier Ferenandez" ;
                   dct:date-accepted "2019-04-05"^^xsd:date ;
                   dct:description "The class of Data Controllers that control this particular data handling, any legal entity that is defined by article 4.7 of GDPR."@en ;
                   rdfs:isDefinedBy <https://eur-lex.europa.eu/eli/reg/2016/679/art_4/par_7/pnt_g/oj> ;
                   sw:term_status "accepted" .


###  http://w3.org/ns/dpv#DataProcessor
dpv:DataProcessor rdf:type owl:Class ;
                  rdfs:subClassOf dpv:Recipient ;
                  dct:created "2019-06-04"^^xsd:date ;
                  dct:creator "Harshvardhan J. Pandit" ;
                  dct:date-accepted "2019-06-04"^^xsd:date ;
                  dct:description "‘processor’ means a natural or legal person, public authority, agency or other body which processes personal data on behalf of the controller;"@en ;
                  rdfs:isDefinedBy <https://eur-lex.europa.eu/eli/reg/2016/679/art_4/par_8/pnt_g/oj> ;
                  sw:term_status "approved" .


###  http://w3.org/ns/dpv#DataSubject
dpv:DataSubject rdf:type owl:Class ;
                dct:created "2019-04-04"^^xsd:date ;
                dct:creator "Axel Polleres, Javier Ferenandez" ;
                dct:date-accepted "2019-04-05"^^xsd:date ;
                dct:description "The class of Data Subject that this particular data handling applies to, any legal entity that is defined by article 4.1 of GDPR."@en ;
                rdfs:isDefinedBy <https://eur-lex.europa.eu/eli/reg/2016/679/art_4/par_1/pnt_g/oj> ;
                sw:term_status "accepted" .


###  http://w3.org/ns/dpv#DeIdentification
dpv:DeIdentification rdf:type owl:Class ;
                     rdfs:subClassOf dpv:PseudoAnonymization ;
                     dct:created "2019-04-04"^^xsd:date ;
                     dct:creator "Axel Polleres, Rob Brennan, Harshvardhan J. Pandit, Mark Lizar" ;
                     dct:date-accepted "2019-04-05"^^xsd:date ;
                     dct:description "Process by identifiable personal data (PII) is converted to un-identifiable personal data"@en ;
                     rdfs:isDefinedBy "DPVCG" ;
                     sw:term_status "accepted" .


###  http://w3.org/ns/dpv#DeliveryOfGoods
dpv:DeliveryOfGoods rdf:type owl:Class ;
                    rdfs:subClassOf dpv:ServiceProvision ;
                    dct:created "2018-12-10"^^xsd:date ;
                    dct:creator "Harshvardhan J. Pandit, Javier Fernandez, Axel Polleres, Elmar Kiesling, Fajar Ekaputra, Simon Steyskal" ;
                    dct:date-accepted "2019-04-05"^^xsd:date ;
                    dct:description "To deliver goods and services"@en ;
                    rdfs:isDefinedBy <https://www.w3.org/community/dpvcg/wiki/Purposes_for_handling_Personal_Data#High-level_categories_.28to-be-discussed.29> ;
                    rdfs:seeAlso svpu:Delivery ;
                    sw:term_status "accepted" .


###  http://w3.org/ns/dpv#Demeanor
dpv:Demeanor rdf:type owl:Class ;
             rdfs:subClassOf dpv:Behavioral ;
             dct:created "2019-04-04"^^xsd:date ;
             dct:creator "Elmar; Harshvardhan J. Pandit, Fajar" ;
             dct:date-accepted "2019-06-04"^^xsd:date ;
             dct:description "Information that relates to an individual's demeanor."@en ;
             rdfs:isDefinedBy <https://enterprivacy.com/wp-content/uploads/2018/09/Categories-of-Personal-Information.pdf> ;
             sw:term_status "accepted" .


###  http://w3.org/ns/dpv#Demographic
dpv:Demographic rdf:type owl:Class ;
                rdfs:subClassOf dpv:External ;
                dct:created "2019-04-04"^^xsd:date ;
                dct:creator "Elmar; Harshvardhan J. Pandit, Fajar" ;
                dct:date-accepted "2019-06-04"^^xsd:date ;
                dct:description "Information that describes an individual’s characteristics shared with others"@en ;
                rdfs:isDefinedBy <https://enterprivacy.com/wp-content/uploads/2018/09/Categories-of-Personal-Information.pdf> ;
                sw:term_status "accepted" .


###  http://w3.org/ns/dpv#Derive
dpv:Derive rdf:type owl:Class ;
           rdfs:subClassOf dpv:Transform ;
           dct:created "2019-04-04"^^xsd:date ;
           dct:date-accepted "2019-05-07"^^xsd:date ;
           dct:description "to create new derivative data from the original data"@en ;
           rdfs:isDefinedBy <https://www.specialprivacy.eu/vocabs/processing> ;
           rdfs:seeAlso svpr:Derive ;
           sw:term_status "accepted" .


###  http://w3.org/ns/dpv#DerivedPersonalData
dpv:DerivedPersonalData rdf:type owl:Class ;
                        rdfs:subClassOf dpv:PersonalDataCategory ;
                        dct:created "2019-05-07"^^xsd:date ;
                        dct:creator "Elmar; Harshvardhan J. Pandit, Fajar" ;
                        dct:date-accepted "2019-05-07"^^xsd:date ;
                        dct:description "Derived data is data that has not been directly provided by the DataSubject, but has been derived from other collected or externally obtained data."@en ;
                        rdfs:seeAlso svd:Derived ;
                        sw:term_status "accepted" .


###  http://w3.org/ns/dpv#DesignStandard
dpv:DesignStandard rdf:type owl:Class ;
                   rdfs:subClassOf dpv:GuidelinesPrinciple ;
                   dct:created "2019-04-04"^^xsd:date ;
                   dct:creator "Axel Polleres, Rob Brennan, Harshvardhan J. Pandit, Mark Lizar" ;
                   dct:date-accepted "2019-04-05"^^xsd:date ;
                   dct:description "A set of rules or guidelines outlining criterias for design"@en ;
                   rdfs:isDefinedBy "DPVCG" ;
                   sw:term_status "accepted" .


###  http://w3.org/ns/dpv#Destruct
dpv:Destruct rdf:type owl:Class ;
             rdfs:subClassOf dpv:Remove ;
             dct:created "2019-04-04"^^xsd:date ;
             dct:date-accepted "2019-05-07"^^xsd:date ;
             dct:description "to process data in a way it no longer exists or cannot be repaired"@en ;
             rdfs:isDefinedBy <https://eur-lex.europa.eu/eli/reg/2016/679/art_4/par_2/oj> ;
             sw:term_status "accepted" .


###  http://w3.org/ns/dpv#DeviceBased
dpv:DeviceBased rdf:type owl:Class ;
                rdfs:subClassOf dpv:Tracking ;
                dct:created "2019-04-04"^^xsd:date ;
                dct:creator "Elmar; Harshvardhan J. Pandit, Fajar" ;
                dct:date-accepted "2019-06-04"^^xsd:date ;
                dct:description "Information about a device that an individual uses for personal use (even part-time or with others)"@en ;
                rdfs:isDefinedBy <https://enterprivacy.com/wp-content/uploads/2018/09/Categories-of-Personal-Information.pdf> ;
                rdfs:seeAlso svd:Computer ;
                sw:term_status "accepted" .


###  http://w3.org/ns/dpv#Dialect
dpv:Dialect rdf:type owl:Class ;
            rdfs:subClassOf dpv:Language ;
            dct:created "2019-04-04"^^xsd:date ;
            dct:creator "Elmar; Harshvardhan J. Pandit, Fajar" ;
            dct:date-accepted "2019-06-04"^^xsd:date ;
            dct:description "Information about an individual’s dialect."@en ;
            rdfs:isDefinedBy <https://enterprivacy.com/wp-content/uploads/2018/09/Categories-of-Personal-Information.pdf> ;
            sw:term_status "accepted" .


###  http://w3.org/ns/dpv#Disability
dpv:Disability rdf:type owl:Class ;
               rdfs:subClassOf dpv:MedicalHealth ;
               dct:created "2019-04-04"^^xsd:date ;
               dct:creator "Elmar; Harshvardhan J. Pandit, Fajar" ;
               dct:date-accepted "2019-06-04"^^xsd:date ;
               dct:description "Information about an individual's disabilities."@en ;
               rdfs:isDefinedBy <https://enterprivacy.com/wp-content/uploads/2018/09/Categories-of-Personal-Information.pdf> ;
               sw:term_status "accepted" .


###  http://w3.org/ns/dpv#DisciplinaryAction
dpv:DisciplinaryAction rdf:type owl:Class ;
                       rdfs:subClassOf dpv:Professional ;
                       dct:created "2019-04-04"^^xsd:date ;
                       dct:creator "Elmar; Harshvardhan J. Pandit, Fajar" ;
                       dct:date-accepted "2019-06-04"^^xsd:date ;
                       dct:description "Information about disciplinary actions associated with an individual"@en ;
                       rdfs:isDefinedBy <https://enterprivacy.com/wp-content/uploads/2018/09/Categories-of-Personal-Information.pdf> ;
                       sw:term_status "accepted" .


###  http://w3.org/ns/dpv#Disclose
dpv:Disclose rdf:type owl:Class ;
             rdfs:subClassOf dpv:Processing ;
             dct:created "2019-04-04"^^xsd:date ;
             dct:date-accepted "2019-05-07"^^xsd:date ;
             dct:description "to make data known"@en ;
             rdfs:isDefinedBy "DPVCG" ;
             sw:term_status "accepted" .


###  http://w3.org/ns/dpv#DiscloseByTransmission
dpv:DiscloseByTransmission rdf:type owl:Class ;
                           rdfs:subClassOf dpv:Disclose ;
                           dct:created "2019-04-04"^^xsd:date ;
                           dct:date-accepted "2019-05-07"^^xsd:date ;
                           dct:description "to disclose data by means of transmission"@en ;
                           rdfs:isDefinedBy <https://eur-lex.europa.eu/eli/reg/2016/679/art_4/par_2/oj> ;
                           sw:term_status "accepted" .


###  http://w3.org/ns/dpv#Dislike
dpv:Dislike rdf:type owl:Class ;
            rdfs:subClassOf dpv:Interest ;
            dct:created "2019-04-04"^^xsd:date ;
            dct:creator "Elmar; Harshvardhan J. Pandit, Fajar" ;
            dct:date-accepted "2019-06-04"^^xsd:date ;
            dct:description "Information relating to a user's dislikes."@en ;
            rdfs:isDefinedBy <https://enterprivacy.com/wp-content/uploads/2018/09/Categories-of-Personal-Information.pdf> ;
            sw:term_status "accepted" .


###  http://w3.org/ns/dpv#Disseminate
dpv:Disseminate rdf:type owl:Class ;
                rdfs:subClassOf dpv:Disclose ;
                dct:created "2019-04-04"^^xsd:date ;
                dct:date-accepted "2019-05-07"^^xsd:date ;
                dct:description "to spread data throughout"@en ;
                rdfs:isDefinedBy <https://eur-lex.europa.eu/eli/reg/2016/679/art_4/par_2/oj> ;
                sw:term_status "accepted" .


###  http://w3.org/ns/dpv#Divorce
dpv:Divorce rdf:type owl:Class ;
            rdfs:subClassOf dpv:FamilyStructure ;
            dct:created "2019-04-04"^^xsd:date ;
            dct:creator "Elmar; Harshvardhan J. Pandit, Fajar" ;
            dct:date-accepted "2019-06-04"^^xsd:date ;
            dct:description "Information about an individual's divorce(s)."@en ;
            rdfs:isDefinedBy <https://enterprivacy.com/wp-content/uploads/2018/09/Categories-of-Personal-Information.pdf> ;
            sw:term_status "accepted" .


###  http://w3.org/ns/dpv#DrugTestResult
dpv:DrugTestResult rdf:type owl:Class ;
                   rdfs:subClassOf dpv:MedicalHealth ;
                   dct:created "2019-04-04"^^xsd:date ;
                   dct:creator "Elmar; Harshvardhan J. Pandit, Fajar" ;
                   dct:date-accepted "2019-06-04"^^xsd:date ;
                   dct:description "Information about an individual's drug test results."@en ;
                   rdfs:isDefinedBy <https://enterprivacy.com/wp-content/uploads/2018/09/Categories-of-Personal-Information.pdf> ;
                   sw:term_status "accepted" .


###  http://w3.org/ns/dpv#EmailAddress
dpv:EmailAddress rdf:type owl:Class ;
                 rdfs:subClassOf dpv:Contact ;
                 dct:created "2019-04-04"^^xsd:date ;
                 dct:creator "Elmar; Harshvardhan J. Pandit, Fajar" ;
                 dct:date-accepted "2019-06-04"^^xsd:date ;
                 dct:description "Information about an individual's Email address."@en ;
                 rdfs:isDefinedBy <https://enterprivacy.com/wp-content/uploads/2018/09/Categories-of-Personal-Information.pdf> ;
                 sw:term_status "accepted" .


###  http://w3.org/ns/dpv#EmailContent
dpv:EmailContent rdf:type owl:Class ;
                 rdfs:subClassOf dpv:Communication ;
                 dct:created "2019-04-04"^^xsd:date ;
                 dct:creator "Elmar; Harshvardhan J. Pandit, Fajar" ;
                 dct:date-accepted "2019-06-04"^^xsd:date ;
                 dct:description "The contents of Emails that an individual sends or receives."@en ;
                 rdfs:isDefinedBy <https://enterprivacy.com/wp-content/uploads/2018/09/Categories-of-Personal-Information.pdf> ;
                 sw:term_status "accepted" .


###  http://w3.org/ns/dpv#EmploymentHistory
dpv:EmploymentHistory rdf:type owl:Class ;
                      rdfs:subClassOf dpv:Professional ;
                      dct:created "2019-04-04"^^xsd:date ;
                      dct:creator "Elmar; Harshvardhan J. Pandit, Fajar" ;
                      dct:date-accepted "2019-06-04"^^xsd:date ;
                      dct:description "Information about an individual's employment history"@en ;
                      rdfs:isDefinedBy <https://enterprivacy.com/wp-content/uploads/2018/09/Categories-of-Personal-Information.pdf> ;
                      sw:term_status "accepted" .


###  http://w3.org/ns/dpv#EncryptionInRest
dpv:EncryptionInRest rdf:type owl:Class ;
                     rdfs:subClassOf dpv:PseudonymisationEncryption ;
                     dct:created "2019-04-04"^^xsd:date ;
                     dct:creator "Axel Polleres, Rob Brennan, Harshvardhan J. Pandit, Mark Lizar" ;
                     dct:date-accepted "2019-04-05"^^xsd:date ;
                     dct:description "Encryption of data when being stored (persistent encryption)"@en ;
                     rdfs:isDefinedBy "DPVCG" ;
                     sw:term_status "accepted" .


###  http://w3.org/ns/dpv#EncryptionInTransfer
dpv:EncryptionInTransfer rdf:type owl:Class ;
                         rdfs:subClassOf dpv:PseudonymisationEncryption ;
                         dct:created "2019-04-04"^^xsd:date ;
                         dct:creator "Axel Polleres, Rob Brennan, Harshvardhan J. Pandit, Mark Lizar" ;
                         dct:date-accepted "2019-04-05"^^xsd:date ;
                         dct:description "Encryption of data in transit e.g. when being transferred from one location to another, including sharing"@en ;
                         rdfs:isDefinedBy "DPVCG" ;
                         sw:term_status "accepted" .


###  http://w3.org/ns/dpv#Erase
dpv:Erase rdf:type owl:Class ;
          rdfs:subClassOf dpv:Remove ;
          dct:created "2019-04-04"^^xsd:date ;
          dct:date-accepted "2019-05-07"^^xsd:date ;
          dct:description "to delete data"@en ;
          rdfs:isDefinedBy <https://eur-lex.europa.eu/eli/reg/2016/679/art_4/par_2/oj> ;
          sw:term_status "accepted" .


###  http://w3.org/ns/dpv#EthnicOrigin
dpv:EthnicOrigin rdf:type owl:Class ;
                 rdfs:subClassOf dpv:Ethnicity ,
                                 dpv:SpecialCategoryPersonalData ;
                 dct:created "2019-04-04"^^xsd:date ;
                 dct:creator "Elmar; Harshvardhan J. Pandit, Fajar" ;
                 dct:date-accepted "2019-06-04"^^xsd:date ;
                 dct:description "Information related to an individual's ethnic origin."@en ;
                 rdfs:isDefinedBy <https://enterprivacy.com/wp-content/uploads/2018/09/Categories-of-Personal-Information.pdf> ;
                 sw:term_status "accepted" .


###  http://w3.org/ns/dpv#Ethnicity
dpv:Ethnicity rdf:type owl:Class ;
              rdfs:subClassOf dpv:External ;
              dct:created "2019-04-04"^^xsd:date ;
              dct:creator "Elmar; Harshvardhan J. Pandit, Fajar" ;
              dct:date-accepted "2019-06-04"^^xsd:date ;
              dct:description "Information that describes an individual’s origins and lineage"@en ;
              rdfs:isDefinedBy <https://enterprivacy.com/wp-content/uploads/2018/09/Categories-of-Personal-Information.pdf> ;
              sw:term_status "accepted" .


###  http://w3.org/ns/dpv#External
dpv:External rdf:type owl:Class ;
             rdfs:subClassOf dpv:PersonalDataCategory ;
             dct:created "2019-04-04"^^xsd:date ;
             dct:creator "Elmar; Harshvardhan J. Pandit, Fajar" ;
             dct:date-accepted "2019-06-04"^^xsd:date ;
             dct:description "Personal Data that can be observed by another person i.e. has external characteristics that make it visible"@en ;
             rdfs:isDefinedBy <https://enterprivacy.com/wp-content/uploads/2018/09/Categories-of-Personal-Information.pdf> ;
             sw:term_status "accepted" .


###  http://w3.org/ns/dpv#Family
dpv:Family rdf:type owl:Class ;
           rdfs:subClassOf dpv:Social ;
           dct:created "2019-04-04"^^xsd:date ;
           dct:creator "Elmar; Harshvardhan J. Pandit, Fajar" ;
           dct:date-accepted "2019-06-04"^^xsd:date ;
           dct:description "Information about an individual’s family and relationships"@en ;
           rdfs:isDefinedBy <https://enterprivacy.com/wp-content/uploads/2018/09/Categories-of-Personal-Information.pdf> ;
           sw:term_status "accepted" .


###  http://w3.org/ns/dpv#FamilyHealthHistory
dpv:FamilyHealthHistory rdf:type owl:Class ;
                        rdfs:subClassOf dpv:HealthHistory ;
                        dct:created "2019-04-04"^^xsd:date ;
                        dct:creator "Elmar; Harshvardhan J. Pandit, Fajar" ;
                        dct:date-accepted "2019-06-04"^^xsd:date ;
                        dct:description "Information related to an individual's family health history."@en ;
                        rdfs:isDefinedBy <https://enterprivacy.com/wp-content/uploads/2018/09/Categories-of-Personal-Information.pdf> ;
                        sw:term_status "accepted" .


###  http://w3.org/ns/dpv#FamilyStructure
dpv:FamilyStructure rdf:type owl:Class ;
                    rdfs:subClassOf dpv:Family ;
                    dct:created "2019-04-04"^^xsd:date ;
                    dct:creator "Elmar; Harshvardhan J. Pandit, Fajar" ;
                    dct:date-accepted "2019-06-04"^^xsd:date ;
                    dct:description "Information that describes an individual's family structure."@en ;
                    rdfs:isDefinedBy <https://enterprivacy.com/wp-content/uploads/2018/09/Categories-of-Personal-Information.pdf> ;
                    sw:term_status "accepted" .


###  http://w3.org/ns/dpv#Favorite
dpv:Favorite rdf:type owl:Class ;
             rdfs:subClassOf dpv:Preference ;
             dct:created "2019-04-04"^^xsd:date ;
             dct:creator "Elmar; Harshvardhan J. Pandit, Fajar" ;
             dct:date-accepted "2019-06-04"^^xsd:date ;
             dct:description "Information about an individual's favorites"@en ;
             rdfs:isDefinedBy <https://enterprivacy.com/wp-content/uploads/2018/09/Categories-of-Personal-Information.pdf> ;
             sw:term_status "accepted" .


###  http://w3.org/ns/dpv#FavoriteColor
dpv:FavoriteColor rdf:type owl:Class ;
                  rdfs:subClassOf dpv:Favorite ;
                  dct:created "2019-04-04"^^xsd:date ;
                  dct:creator "Elmar; Harshvardhan J. Pandit, Fajar" ;
                  dct:date-accepted "2019-06-04"^^xsd:date ;
                  dct:description "Information about an individual's favorite color."@en ;
                  rdfs:isDefinedBy <https://enterprivacy.com/wp-content/uploads/2018/09/Categories-of-Personal-Information.pdf> ;
                  sw:term_status "accepted" .


###  http://w3.org/ns/dpv#FavoriteFood
dpv:FavoriteFood rdf:type owl:Class ;
                 rdfs:subClassOf dpv:Favorite ;
                 dct:created "2019-04-04"^^xsd:date ;
                 dct:creator "Elmar; Harshvardhan J. Pandit, Fajar" ;
                 dct:date-accepted "2019-06-04"^^xsd:date ;
                 dct:description "Information about an individual's favorite food."@en ;
                 rdfs:isDefinedBy <https://enterprivacy.com/wp-content/uploads/2018/09/Categories-of-Personal-Information.pdf> ;
                 sw:term_status "accepted" .


###  http://w3.org/ns/dpv#FavoriteMusic
dpv:FavoriteMusic rdf:type owl:Class ;
                  rdfs:subClassOf dpv:Favorite ;
                  dct:created "2019-04-04"^^xsd:date ;
                  dct:creator "Elmar; Harshvardhan J. Pandit, Fajar" ;
                  dct:date-accepted "2019-06-04"^^xsd:date ;
                  dct:description "Information about an individual's favorite music."@en ;
                  rdfs:isDefinedBy <https://enterprivacy.com/wp-content/uploads/2018/09/Categories-of-Personal-Information.pdf> ;
                  sw:term_status "accepted" .


###  http://w3.org/ns/dpv#Fetish
dpv:Fetish rdf:type owl:Class ;
           rdfs:subClassOf dpv:Sexual ;
           dct:created "2019-04-04"^^xsd:date ;
           dct:creator "Elmar; Harshvardhan J. Pandit, Fajar" ;
           dct:date-accepted "2019-06-04"^^xsd:date ;
           dct:description "Information an individual's sexual fetishes"@en ;
           rdfs:isDefinedBy <https://enterprivacy.com/wp-content/uploads/2018/09/Categories-of-Personal-Information.pdf> ;
           sw:term_status "accepted" .


###  http://w3.org/ns/dpv#Financial
dpv:Financial rdf:type owl:Class ;
              rdfs:subClassOf dpv:PersonalDataCategory ;
              dct:created "2019-04-04"^^xsd:date ;
              dct:creator "Elmar; Harshvardhan J. Pandit, Fajar" ;
              dct:date-accepted "2019-06-04"^^xsd:date ;
              dct:description "Personal data regarding finance or monetary information"@en ;
              rdfs:isDefinedBy <https://enterprivacy.com/wp-content/uploads/2018/09/Categories-of-Personal-Information.pdf> ;
              rdfs:seeAlso svd:Financial ;
              sw:term_status "accepted" .


###  http://w3.org/ns/dpv#FinancialAccount
dpv:FinancialAccount rdf:type owl:Class ;
                     rdfs:subClassOf dpv:Financial ;
                     dct:created "2019-04-04"^^xsd:date ;
                     dct:creator "Elmar; Harshvardhan J. Pandit, Fajar" ;
                     dct:date-accepted "2019-06-04"^^xsd:date ;
                     dct:description "Information that identifies an individual’s financial account"@en ;
                     rdfs:isDefinedBy <https://enterprivacy.com/wp-content/uploads/2018/09/Categories-of-Personal-Information.pdf> ;
                     sw:term_status "accepted" .


###  http://w3.org/ns/dpv#FinancialAccountNumber
dpv:FinancialAccountNumber rdf:type owl:Class ;
                           rdfs:subClassOf dpv:AccountIdentifier ;
                           dct:created "2019-04-04"^^xsd:date ;
                           dct:creator "Elmar; Harshvardhan J. Pandit, Fajar" ;
                           dct:date-accepted "2019-06-04"^^xsd:date ;
                           dct:description "Information about an individual's financial account number"@en ;
                           rdfs:isDefinedBy <https://enterprivacy.com/wp-content/uploads/2018/09/Categories-of-Personal-Information.pdf> ;
                           sw:term_status "accepted" .


###  http://w3.org/ns/dpv#Fingerprint
dpv:Fingerprint rdf:type owl:Class ;
                rdfs:subClassOf dpv:Biometric ;
                dct:created "2019-04-04"^^xsd:date ;
                dct:creator "Elmar; Harshvardhan J. Pandit, Fajar" ;
                dct:date-accepted "2019-06-04"^^xsd:date ;
                dct:description "Information related to an individual's fingerprint used for biometric purposes."@en ;
                rdfs:isDefinedBy <https://enterprivacy.com/wp-content/uploads/2018/09/Categories-of-Personal-Information.pdf> ;
                sw:term_status "accepted" .


###  http://w3.org/ns/dpv#FraudPreventionAndDetection
dpv:FraudPreventionAndDetection rdf:type owl:Class ;
                                rdfs:subClassOf dpv:Security ;
                                dct:created "2018-12-10"^^xsd:date ;
                                dct:creator "Harshvardhan J. Pandit, Javier Fernandez, Axel Polleres, Elmar Kiesling, Fajar Ekaputra, Simon Steyskal" ;
                                dct:date-accepted "2019-04-05"^^xsd:date ;
                                dct:description "To detect and prevent fraud"@en ;
                                rdfs:isDefinedBy <https://www.w3.org/community/dpvcg/wiki/Purposes_for_handling_Personal_Data#High-level_categories_.28to-be-discussed.29> ;
                                rdfs:seeAlso svpu:Government ;
                                sw:term_status "accepted" .


###  http://w3.org/ns/dpv#Friend
dpv:Friend rdf:type owl:Class ;
           rdfs:subClassOf dpv:SocialNetwork ;
           dct:created "2019-04-04"^^xsd:date ;
           dct:creator "Elmar; Harshvardhan J. Pandit, Fajar" ;
           dct:date-accepted "2019-06-04"^^xsd:date ;
           dct:description "Information about friends of the individual in a social network. Includes aspects of friendships such as years together or nature of friendship."@en ;
           rdfs:isDefinedBy <https://enterprivacy.com/wp-content/uploads/2018/09/Categories-of-Personal-Information.pdf> ;
           sw:term_status "accepted" .


###  http://w3.org/ns/dpv#GPSCoordinate
dpv:GPSCoordinate rdf:type owl:Class ;
                  rdfs:subClassOf dpv:Location ;
                  dct:created "2019-04-04"^^xsd:date ;
                  dct:creator "Elmar; Harshvardhan J. Pandit, Fajar" ;
                  dct:date-accepted "2019-06-04"^^xsd:date ;
                  dct:description "Global position system coordinates of a user's location."@en ;
                  rdfs:isDefinedBy <https://enterprivacy.com/wp-content/uploads/2018/09/Categories-of-Personal-Information.pdf> ;
                  sw:term_status "accepted" .


###  http://w3.org/ns/dpv#Gender
dpv:Gender rdf:type owl:Class ;
           rdfs:subClassOf dpv:PhysicalCharacteristic ;
           dct:created "2019-04-04"^^xsd:date ;
           dct:creator "Elmar; Harshvardhan J. Pandit, Fajar" ;
           dct:date-accepted "2019-06-04"^^xsd:date ;
           dct:description "Information about an individual's gender"@en ;
           rdfs:isDefinedBy <https://enterprivacy.com/wp-content/uploads/2018/09/Categories-of-Personal-Information.pdf> ;
           sw:term_status "accepted" .


###  http://w3.org/ns/dpv#GeneralReputation
dpv:GeneralReputation rdf:type owl:Class ;
                      rdfs:subClassOf dpv:PublicLife ;
                      dct:created "2019-04-04"^^xsd:date ;
                      dct:creator "Elmar; Harshvardhan J. Pandit, Fajar" ;
                      dct:date-accepted "2019-06-04"^^xsd:date ;
                      dct:description "Information about an individual's reputation in the public sphere"@en ;
                      rdfs:isDefinedBy <https://enterprivacy.com/wp-content/uploads/2018/09/Categories-of-Personal-Information.pdf> ;
                      sw:term_status "accepted" .


###  http://w3.org/ns/dpv#Geographic
dpv:Geographic rdf:type owl:Class ;
               rdfs:subClassOf dpv:Demographic ;
               dct:created "2019-04-04"^^xsd:date ;
               dct:creator "Elmar; Harshvardhan J. Pandit, Fajar" ;
               dct:date-accepted "2019-06-04"^^xsd:date ;
               dct:description "Geographic information relating to an individual (e.g., home address)"@en ;
               rdfs:isDefinedBy <https://enterprivacy.com/wp-content/uploads/2018/09/Categories-of-Personal-Information.pdf> ;
               sw:term_status "accepted" .


###  http://w3.org/ns/dpv#GroupMembership
dpv:GroupMembership rdf:type owl:Class ;
                    rdfs:subClassOf dpv:SocialNetwork ;
                    dct:created "2019-04-04"^^xsd:date ;
                    dct:creator "Elmar; Harshvardhan J. Pandit, Fajar" ;
                    dct:date-accepted "2019-06-04"^^xsd:date ;
                    dct:description "Information about groups the individual is included or associated with in a social network"@en ;
                    rdfs:isDefinedBy <https://enterprivacy.com/wp-content/uploads/2018/09/Categories-of-Personal-Information.pdf> ;
                    sw:term_status "accepted" .


###  http://w3.org/ns/dpv#GuidelinesPrinciple
dpv:GuidelinesPrinciple rdf:type owl:Class ;
                        rdfs:subClassOf dpv:OrganisationalMeasure ;
                        dct:created "2019-04-04"^^xsd:date ;
                        dct:creator "Axel Polleres, Rob Brennan, Harshvardhan J. Pandit, Mark Lizar" ;
                        dct:date-accepted "2019-04-05"^^xsd:date ;
                        dct:description "Guidelines or Principles regarding processing and operational measures"@en ;
                        rdfs:isDefinedBy "DPVCG" ;
                        sw:term_status "accepted" .


###  http://w3.org/ns/dpv#HairColor
dpv:HairColor rdf:type owl:Class ;
              rdfs:subClassOf dpv:PhysicalCharacteristic ;
              dct:created "2019-04-04"^^xsd:date ;
              dct:creator "Elmar; Harshvardhan J. Pandit, Fajar" ;
              dct:date-accepted "2019-06-04"^^xsd:date ;
              dct:description "Information about an individual's hair colour"@en ;
              rdfs:isDefinedBy <https://enterprivacy.com/wp-content/uploads/2018/09/Categories-of-Personal-Information.pdf> ;
              sw:term_status "accepted" .


###  http://w3.org/ns/dpv#Health
dpv:Health rdf:type owl:Class ;
           rdfs:subClassOf dpv:MedicalHealth ;
           dct:created "2019-04-04"^^xsd:date ;
           dct:creator "Elmar; Harshvardhan J. Pandit, Fajar" ;
           dct:date-accepted "2019-06-04"^^xsd:date ;
           dct:description "Information about an individual's health."@en ;
           rdfs:isDefinedBy <https://enterprivacy.com/wp-content/uploads/2018/09/Categories-of-Personal-Information.pdf> ;
           rdfs:seeAlso svd:Health ;
           sw:term_status "accepted" .


###  http://w3.org/ns/dpv#HealthHistory
dpv:HealthHistory rdf:type owl:Class ;
                  rdfs:subClassOf dpv:MedicalHealth ;
                  dct:created "2019-04-04"^^xsd:date ;
                  dct:creator "Elmar; Harshvardhan J. Pandit, Fajar" ;
                  dct:date-accepted "2019-06-04"^^xsd:date ;
                  dct:description "Information about an individual's health history."@en ;
                  rdfs:isDefinedBy <https://enterprivacy.com/wp-content/uploads/2018/09/Categories-of-Personal-Information.pdf> ;
                  sw:term_status "accepted" .


###  http://w3.org/ns/dpv#HealthRecord
dpv:HealthRecord rdf:type owl:Class ;
                 rdfs:subClassOf dpv:MedicalHealth ;
                 dct:created "2019-04-04"^^xsd:date ;
                 dct:creator "Elmar; Harshvardhan J. Pandit, Fajar" ;
                 dct:date-accepted "2019-06-04"^^xsd:date ;
                 dct:description "Information about an individual's health record."@en ;
                 rdfs:isDefinedBy <https://enterprivacy.com/wp-content/uploads/2018/09/Categories-of-Personal-Information.pdf> ;
                 sw:term_status "accepted" .


###  http://w3.org/ns/dpv#Height
dpv:Height rdf:type owl:Class ;
           rdfs:subClassOf dpv:PhysicalCharacteristic ;
           dct:created "2019-04-04"^^xsd:date ;
           dct:creator "Elmar; Harshvardhan J. Pandit, Fajar" ;
           dct:date-accepted "2019-06-04"^^xsd:date ;
           dct:description "Information about an individual's physical height"@en ;
           rdfs:isDefinedBy <https://enterprivacy.com/wp-content/uploads/2018/09/Categories-of-Personal-Information.pdf> ;
           sw:term_status "accepted" .


###  http://w3.org/ns/dpv#Historical
dpv:Historical rdf:type owl:Class ;
               rdfs:subClassOf dpv:PersonalDataCategory ;
               dct:created "2019-04-04"^^xsd:date ;
               dct:creator "Elmar; Harshvardhan J. Pandit, Fajar" ;
               dct:date-accepted "2019-06-04"^^xsd:date ;
               dct:description "Historical personal data is that which is related to or relevant for history or past events in the context of the person or their life."@en ;
               rdfs:isDefinedBy <https://enterprivacy.com/wp-content/uploads/2018/09/Categories-of-Personal-Information.pdf> ;
               sw:term_status "accepted" .


###  http://w3.org/ns/dpv#HouseOwned
dpv:HouseOwned rdf:type owl:Class ;
               rdfs:subClassOf dpv:Ownership ;
               dct:created "2019-04-04"^^xsd:date ;
               dct:creator "Elmar; Harshvardhan J. Pandit, Fajar" ;
               dct:date-accepted "2019-06-04"^^xsd:date ;
               dct:description "Information about house(s) owned by an individual."@en ;
               rdfs:isDefinedBy <https://enterprivacy.com/wp-content/uploads/2018/09/Categories-of-Personal-Information.pdf> ;
               sw:term_status "accepted" .


###  http://w3.org/ns/dpv#IPAddress
dpv:IPAddress rdf:type owl:Class ;
              rdfs:subClassOf dpv:DeviceBased ;
              dct:created "2019-04-04"^^xsd:date ;
              dct:creator "Elmar; Harshvardhan J. Pandit, Fajar" ;
              dct:date-accepted "2019-06-04"^^xsd:date ;
              dct:description "An Internet protocol (IP) address of a device used by an individual."@en ;
              rdfs:isDefinedBy <https://enterprivacy.com/wp-content/uploads/2018/09/Categories-of-Personal-Information.pdf> ;
              sw:term_status "accepted" .


###  http://w3.org/ns/dpv#Identifying
dpv:Identifying rdf:type owl:Class ;
                rdfs:subClassOf dpv:External ;
                dct:created "2019-04-04"^^xsd:date ;
                dct:creator "Elmar; Harshvardhan J. Pandit, Fajar" ;
                dct:date-accepted "2019-06-04"^^xsd:date ;
                dct:description "Information that uniquely or semi-uniquely identifies a specific individual"@en ;
                rdfs:isDefinedBy <https://enterprivacy.com/wp-content/uploads/2018/09/Categories-of-Personal-Information.pdf> ;
                sw:term_status "accepted" .


###  http://w3.org/ns/dpv#IdentityVerification
dpv:IdentityVerification rdf:type owl:Class ;
                         rdfs:subClassOf dpv:Security ;
                         dct:created "2018-12-10"^^xsd:date ;
                         dct:creator "Harshvardhan J. Pandit, Javier Fernandez, Axel Polleres, Elmar Kiesling, Fajar Ekaputra, Simon Steyskal" ;
                         dct:date-accepted "2019-04-05"^^xsd:date ;
                         dct:description "To verify and authorise identity"@en ;
                         rdfs:isDefinedBy <https://www.w3.org/community/dpvcg/wiki/Purposes_for_handling_Personal_Data#High-level_categories_.28to-be-discussed.29> ;
                         sw:term_status "accepted" .


###  http://w3.org/ns/dpv#ImproveExistingProductsAndServices
dpv:ImproveExistingProductsAndServices rdf:type owl:Class ;
                                       rdfs:subClassOf dpv:OptimisationForController ;
                                       dct:created "2018-12-10"^^xsd:date ;
                                       dct:creator "Harshvardhan J. Pandit, Javier Fernandez, Axel Polleres, Elmar Kiesling, Fajar Ekaputra, Simon Steyskal" ;
                                       dct:date-accepted "2019-04-05"^^xsd:date ;
                                       dct:description "To improve existing products and services"@en ;
                                       rdfs:isDefinedBy <https://www.w3.org/community/dpvcg/wiki/Purposes_for_handling_Personal_Data#High-level_categories_.28to-be-discussed.29> ;
                                       sw:term_status "accepted" .


###  http://w3.org/ns/dpv#ImproveInternalCRMProcesses
dpv:ImproveInternalCRMProcesses rdf:type owl:Class ;
                                rdfs:subClassOf dpv:OptimisationForController ;
                                dct:created "2018-12-10"^^xsd:date ;
                                dct:creator "Harshvardhan J. Pandit, Javier Fernandez, Axel Polleres, Elmar Kiesling, Fajar Ekaputra, Simon Steyskal" ;
                                dct:date-accepted "2019-04-05"^^xsd:date ;
                                dct:description "To improve customer-relationship management (CRM) processes"@en ;
                                rdfs:isDefinedBy <https://www.w3.org/community/dpvcg/wiki/Purposes_for_handling_Personal_Data#High-level_categories_.28to-be-discussed.29> ;
                                sw:term_status "accepted" .


###  http://w3.org/ns/dpv#Income
dpv:Income rdf:type owl:Class ;
           rdfs:subClassOf dpv:Transactional ;
           dct:created "2019-04-04"^^xsd:date ;
           dct:creator "Elmar; Harshvardhan J. Pandit, Fajar" ;
           dct:date-accepted "2019-06-04"^^xsd:date ;
           dct:description "Information about financial income e.g. for individual or household or family"@en ;
           rdfs:isDefinedBy <https://enterprivacy.com/wp-content/uploads/2018/09/Categories-of-Personal-Information.pdf> ;
           sw:term_status "accepted" .


###  http://w3.org/ns/dpv#IncomeBracket
dpv:IncomeBracket rdf:type owl:Class ;
                  rdfs:subClassOf dpv:Demographic ;
                  dct:created "2019-04-04"^^xsd:date ;
                  dct:creator "Elmar; Harshvardhan J. Pandit, Fajar" ;
                  dct:date-accepted "2019-06-04"^^xsd:date ;
                  dct:description "Information about an individual's income bracket."@en ;
                  rdfs:isDefinedBy <https://enterprivacy.com/wp-content/uploads/2018/09/Categories-of-Personal-Information.pdf> ;
                  sw:term_status "accepted" .


###  http://w3.org/ns/dpv#IncreaseServiceRobustness
dpv:IncreaseServiceRobustness rdf:type owl:Class ;
                              rdfs:subClassOf dpv:OptimisationForController ;
                              dct:created "2018-12-10"^^xsd:date ;
                              dct:creator "Harshvardhan J. Pandit, Javier Fernandez, Axel Polleres, Elmar Kiesling, Fajar Ekaputra, Simon Steyskal" ;
                              dct:date-accepted "2019-04-05"^^xsd:date ;
                              dct:description "To improve the robustness and resilience of services"@en ;
                              rdfs:isDefinedBy <https://www.w3.org/community/dpvcg/wiki/Purposes_for_handling_Personal_Data#High-level_categories_.28to-be-discussed.29> ;
                              sw:term_status "accepted" .


###  http://w3.org/ns/dpv#IndividualHealthHistory
dpv:IndividualHealthHistory rdf:type owl:Class ;
                            rdfs:subClassOf dpv:HealthHistory ;
                            dct:created "2019-04-04"^^xsd:date ;
                            dct:creator "Elmar; Harshvardhan J. Pandit, Fajar" ;
                            dct:date-accepted "2019-06-04"^^xsd:date ;
                            dct:description "Information related to an individual's information health history."@en ;
                            rdfs:isDefinedBy <https://enterprivacy.com/wp-content/uploads/2018/09/Categories-of-Personal-Information.pdf> ;
                            sw:term_status "accepted" .


###  http://w3.org/ns/dpv#Intention
dpv:Intention rdf:type owl:Class ;
              rdfs:subClassOf dpv:Preference ;
              dct:created "2019-04-04"^^xsd:date ;
              dct:creator "Elmar; Harshvardhan J. Pandit, Fajar" ;
              dct:date-accepted "2019-06-04"^^xsd:date ;
              dct:description "Information about an individual's intentions"@en ;
              rdfs:isDefinedBy <https://enterprivacy.com/wp-content/uploads/2018/09/Categories-of-Personal-Information.pdf> ;
              sw:term_status "accepted" .


###  http://w3.org/ns/dpv#Interaction
dpv:Interaction rdf:type owl:Class ;
                rdfs:subClassOf dpv:PublicLife ;
                dct:created "2019-04-04"^^xsd:date ;
                dct:creator "Elmar; Harshvardhan J. Pandit, Fajar" ;
                dct:date-accepted "2019-06-04"^^xsd:date ;
                dct:description "Information about an individual's interactions in the public sphere"@en ;
                rdfs:isDefinedBy <https://enterprivacy.com/wp-content/uploads/2018/09/Categories-of-Personal-Information.pdf> ;
                sw:term_status "accepted" .


###  http://w3.org/ns/dpv#Interest
dpv:Interest rdf:type owl:Class ;
             rdfs:subClassOf dpv:Preference ;
             dct:created "2019-04-04"^^xsd:date ;
             dct:creator "Elmar; Harshvardhan J. Pandit, Fajar" ;
             dct:date-accepted "2019-06-04"^^xsd:date ;
             dct:description "Information about an individual's interests"@en ;
             rdfs:isDefinedBy <https://enterprivacy.com/wp-content/uploads/2018/09/Categories-of-Personal-Information.pdf> ;
             sw:term_status "accepted" .


###  http://w3.org/ns/dpv#Internal
dpv:Internal rdf:type owl:Class ;
             rdfs:subClassOf dpv:PersonalDataCategory ;
             dct:created "2019-04-04"^^xsd:date ;
             dct:creator "Elmar; Harshvardhan J. Pandit, Fajar" ;
             dct:date-accepted "2019-06-04"^^xsd:date ;
             dct:description "Personal data about characteristics of an individual that are internal i.e. cannot be seen or observed"@en ;
             rdfs:isDefinedBy <https://enterprivacy.com/wp-content/uploads/2018/09/Categories-of-Personal-Information.pdf> ;
             sw:term_status "accepted" .


###  http://w3.org/ns/dpv#InternalResourceOptimisation
dpv:InternalResourceOptimisation rdf:type owl:Class ;
                                 rdfs:subClassOf dpv:OptimisationForController ;
                                 dct:created "2018-12-10"^^xsd:date ;
                                 dct:creator "Harshvardhan J. Pandit, Javier Fernandez, Axel Polleres, Elmar Kiesling, Fajar Ekaputra, Simon Steyskal" ;
                                 dct:date-accepted "2019-04-05"^^xsd:date ;
                                 dct:description "Optimisation of internal resources used by the organisation e.g. resource usage"@en ;
                                 rdfs:isDefinedBy <https://www.w3.org/community/dpvcg/wiki/Purposes_for_handling_Personal_Data#High-level_categories_.28to-be-discussed.29> ;
                                 sw:term_status "accepted" .


###  http://w3.org/ns/dpv#Job
dpv:Job rdf:type owl:Class ;
        rdfs:subClassOf dpv:Professional ;
        dct:created "2019-04-04"^^xsd:date ;
        dct:creator "Elmar; Harshvardhan J. Pandit, Fajar" ;
        dct:date-accepted "2019-06-04"^^xsd:date ;
        dct:description "Information about an individual's professional jobs"@en ;
        rdfs:isDefinedBy <https://enterprivacy.com/wp-content/uploads/2018/09/Categories-of-Personal-Information.pdf> ;
        sw:term_status "accepted" .


###  http://w3.org/ns/dpv#KnowledgeBelief
dpv:KnowledgeBelief rdf:type owl:Class ;
                    rdfs:subClassOf dpv:Internal ;
                    dct:created "2019-04-04"^^xsd:date ;
                    dct:creator "Elmar; Harshvardhan J. Pandit, Fajar" ;
                    dct:date-accepted "2019-06-04"^^xsd:date ;
                    dct:description "Information about what a person knows or believes"@en ;
                    rdfs:isDefinedBy <https://enterprivacy.com/wp-content/uploads/2018/09/Categories-of-Personal-Information.pdf> ;
                    sw:term_status "accepted" .


###  http://w3.org/ns/dpv#Language
dpv:Language rdf:type owl:Class ;
             rdfs:subClassOf dpv:Ethnicity ;
             dct:created "2019-04-04"^^xsd:date ;
             dct:creator "Elmar; Harshvardhan J. Pandit, Fajar" ;
             dct:date-accepted "2019-06-04"^^xsd:date ;
             dct:description "Information related to an individual's language."@en ;
             rdfs:isDefinedBy <https://enterprivacy.com/wp-content/uploads/2018/09/Categories-of-Personal-Information.pdf> ;
             sw:term_status "accepted" .


###  http://w3.org/ns/dpv#LegalAgreement
dpv:LegalAgreement rdf:type owl:Class ;
                   rdfs:subClassOf dpv:OrganisationalMeasure ;
                   dct:created "2019-04-04"^^xsd:date ;
                   dct:creator "Axel Polleres, Rob Brennan, Harshvardhan J. Pandit, Mark Lizar" ;
                   dct:date-accepted "2019-04-05"^^xsd:date ;
                   dct:description "A legally binding agreement"@en ;
                   rdfs:isDefinedBy "DPVCG" ;
                   sw:term_status "accepted" .


###  http://w3.org/ns/dpv#LegalBasis
dpv:LegalBasis rdf:type owl:Class ;
               dct:created "2019-04-04"^^xsd:date ;
               dct:date-accepted "2019-04-05"^^xsd:date ;
               dct:description "A particular legal Basis, which permits personal Data handling (e.g. Consent, etc.)"@en ;
               rdfs:isDefinedBy "DPVCG" ;
               sw:term_status "accepted" .


###  http://w3.org/ns/dpv#LegalEntity
dpv:LegalEntity rdf:type owl:Class ;
                rdfs:subClassOf prov:Agent ;
                dct:created "2019-04-04"^^xsd:date ;
                dct:creator "Harshvardhan J. Pandit, Mark Lizar, Bud Bruegger" ;
                dct:date-accepted "2019-04-05"^^xsd:date ;
                dct:description "A Person or Organisation, including Data Subjects, that constitute as a legal entity."@en ;
                sw:term_status "accepted" .


###  http://w3.org/ns/dpv#LifeHistory
dpv:LifeHistory rdf:type owl:Class ;
                rdfs:subClassOf dpv:Historical ;
                dct:created "2019-04-04"^^xsd:date ;
                dct:creator "Elmar; Harshvardhan J. Pandit, Fajar" ;
                dct:date-accepted "2019-06-04"^^xsd:date ;
                dct:description "Information about an individual’s personal history (e.g., events that happened in a person’s life, either to them or just around them which might have influenced them (WWII, 9/11))."@en ;
                rdfs:isDefinedBy <https://enterprivacy.com/wp-content/uploads/2018/09/Categories-of-Personal-Information.pdf> ;
                sw:term_status "accepted" .


###  http://w3.org/ns/dpv#Like
dpv:Like rdf:type owl:Class ;
         rdfs:subClassOf dpv:Interest ;
         dct:created "2019-04-04"^^xsd:date ;
         dct:creator "Elmar; Harshvardhan J. Pandit, Fajar" ;
         dct:date-accepted "2019-06-04"^^xsd:date ;
         dct:description "Information relating to a user's likes."@en ;
         rdfs:isDefinedBy <https://enterprivacy.com/wp-content/uploads/2018/09/Categories-of-Personal-Information.pdf> ;
         sw:term_status "accepted" .


###  http://w3.org/ns/dpv#LinkClicked
dpv:LinkClicked rdf:type owl:Class ;
                rdfs:subClassOf dpv:Behavioral ;
                dct:created "2019-04-04"^^xsd:date ;
                dct:creator "Elmar; Harshvardhan J. Pandit, Fajar" ;
                dct:date-accepted "2019-06-04"^^xsd:date ;
                dct:description "Information on the links that an individual has clicked."@en ;
                rdfs:isDefinedBy <https://enterprivacy.com/wp-content/uploads/2018/09/Categories-of-Personal-Information.pdf> ;
                rdfs:seeAlso svd:Navigation ;
                sw:term_status "accepted" .


###  http://w3.org/ns/dpv#LoanRecord
dpv:LoanRecord rdf:type owl:Class ;
               rdfs:subClassOf dpv:Transactional ;
               dct:created "2019-04-04"^^xsd:date ;
               dct:creator "Elmar; Harshvardhan J. Pandit, Fajar" ;
               dct:date-accepted "2019-06-04"^^xsd:date ;
               dct:description "Information about loans provided or related to the individual"@en ;
               rdfs:isDefinedBy <https://enterprivacy.com/wp-content/uploads/2018/09/Categories-of-Personal-Information.pdf> ;
               sw:term_status "accepted" .


###  http://w3.org/ns/dpv#Location
dpv:Location rdf:type owl:Class ;
             rdfs:subClassOf dpv:Tracking ;
             dct:created "2019-04-04"^^xsd:date ;
             dct:creator "Elmar; Harshvardhan J. Pandit, Fajar" ;
             dct:date-accepted "2019-06-04"^^xsd:date ;
             dct:description "Information about an individual’s location"@en ;
             rdfs:isDefinedBy <https://enterprivacy.com/wp-content/uploads/2018/09/Categories-of-Personal-Information.pdf> ;
             rdfs:seeAlso svd:Location ;
             sw:term_status "accepted" .


###  http://w3.org/ns/dpv#MACAddress
dpv:MACAddress rdf:type owl:Class ;
               rdfs:subClassOf dpv:DeviceBased ;
               dct:created "2019-04-04"^^xsd:date ;
               dct:creator "Elmar; Harshvardhan J. Pandit, Fajar" ;
               dct:date-accepted "2019-06-04"^^xsd:date ;
               dct:description "A Media Access Control (MAC) address of a device used by an individual."@en ;
               rdfs:isDefinedBy <https://enterprivacy.com/wp-content/uploads/2018/09/Categories-of-Personal-Information.pdf> ;
               sw:term_status "accepted" .


###  http://w3.org/ns/dpv#MakeAvailable
dpv:MakeAvailable rdf:type owl:Class ;
                  rdfs:subClassOf dpv:Disclose ;
                  dct:created "2019-04-04"^^xsd:date ;
                  dct:date-accepted "2019-05-07"^^xsd:date ;
                  dct:description "to transform or publish data to be used"@en ;
                  rdfs:isDefinedBy <https://eur-lex.europa.eu/eli/reg/2016/679/art_4/par_2/oj> ;
                  sw:term_status "accepted" .


###  http://w3.org/ns/dpv#MaritalStatus
dpv:MaritalStatus rdf:type owl:Class ;
                  rdfs:subClassOf dpv:PublicLife ;
                  dct:created "2019-04-04"^^xsd:date ;
                  dct:creator "Elmar; Harshvardhan J. Pandit, Fajar" ;
                  dct:date-accepted "2019-06-04"^^xsd:date ;
                  dct:description "Information about an individual's marital status and history"@en ;
                  rdfs:isDefinedBy <https://enterprivacy.com/wp-content/uploads/2018/09/Categories-of-Personal-Information.pdf> ;
                  sw:term_status "accepted" .


###  http://w3.org/ns/dpv#Marriage
dpv:Marriage rdf:type owl:Class ;
             rdfs:subClassOf dpv:FamilyStructure ;
             dct:created "2019-04-04"^^xsd:date ;
             dct:creator "Elmar; Harshvardhan J. Pandit, Fajar" ;
             dct:date-accepted "2019-06-04"^^xsd:date ;
             dct:description "Information about an individual's marriage(s)."@en ;
             rdfs:isDefinedBy <https://enterprivacy.com/wp-content/uploads/2018/09/Categories-of-Personal-Information.pdf> ;
             sw:term_status "accepted" .


###  http://w3.org/ns/dpv#MedicalHealth
dpv:MedicalHealth rdf:type owl:Class ;
                  rdfs:subClassOf dpv:External ,
                                  dpv:SpecialCategoryPersonalData ;
                  dct:created "2019-04-04"^^xsd:date ;
                  dct:creator "Elmar; Harshvardhan J. Pandit, Fajar" ;
                  dct:date-accepted "2019-06-04"^^xsd:date ;
                  dct:description "Information that describes an individual’s health, medical conditions or health care"@en ;
                  rdfs:isDefinedBy <https://enterprivacy.com/wp-content/uploads/2018/09/Categories-of-Personal-Information.pdf> ;
                  sw:term_status "accepted" .


###  http://w3.org/ns/dpv#MentalHealth
dpv:MentalHealth rdf:type owl:Class ;
                 rdfs:subClassOf dpv:Health ;
                 dct:created "2019-04-04"^^xsd:date ;
                 dct:creator "Elmar; Harshvardhan J. Pandit, Fajar" ;
                 dct:date-accepted "2019-06-04"^^xsd:date ;
                 dct:description "Information related to an individual's mental health."@en ;
                 rdfs:isDefinedBy <https://enterprivacy.com/wp-content/uploads/2018/09/Categories-of-Personal-Information.pdf> ;
                 sw:term_status "accepted" .


###  http://w3.org/ns/dpv#Move
dpv:Move rdf:type owl:Class ;
         rdfs:subClassOf dpv:Transfer ;
         dct:created "2019-04-04"^^xsd:date ;
         dct:date-accepted "2019-05-07"^^xsd:date ;
         dct:description "to move data from one location to another including deleting the original copy"@en ;
         rdfs:isDefinedBy <https://www.specialprivacy.eu/vocabs/processing> ;
         rdfs:seeAlso svpr:Move ;
         sw:term_status "accepted" .


###  http://w3.org/ns/dpv#NDA
dpv:NDA rdf:type owl:Class ;
        rdfs:subClassOf dpv:LegalAgreement ;
        dct:created "2019-04-04"^^xsd:date ;
        dct:creator "Axel Polleres, Rob Brennan, Harshvardhan J. Pandit, Mark Lizar" ;
        dct:date-accepted "2019-04-05"^^xsd:date ;
        dct:description "Non-disclosure Agreements e.g. preserving confidentiality of information"@en ;
        rdfs:isDefinedBy "DPVCG" ;
        sw:term_status "accepted" .


###  http://w3.org/ns/dpv#Name
dpv:Name rdf:type owl:Class ;
         rdfs:subClassOf dpv:Identifying ;
         dct:created "2019-04-04"^^xsd:date ;
         dct:creator "Elmar; Harshvardhan J. Pandit, Fajar" ;
         dct:date-accepted "2019-06-04"^^xsd:date ;
         dct:description "A name associated with an individual e.g. given name, nickname."@en ;
         rdfs:isDefinedBy <https://enterprivacy.com/wp-content/uploads/2018/09/Categories-of-Personal-Information.pdf> ;
         sw:term_status "accepted" .


###  http://w3.org/ns/dpv#NonCommercialResearch
dpv:NonCommercialResearch rdf:type owl:Class ;
                          rdfs:subClassOf dpv:ResearchAndDevelopment ;
                          dct:created "2018-12-10"^^xsd:date ;
                          dct:creator "Harshvardhan J. Pandit, Javier Fernandez, Axel Polleres, Elmar Kiesling, Fajar Ekaputra, Simon Steyskal" ;
                          dct:date-accepted "2019-04-05"^^xsd:date ;
                          dct:description "Research conducted in a non-commercial setting e.g. for a non-profit-organisation (NGO)"@en ;
                          rdfs:isDefinedBy <https://www.w3.org/community/dpvcg/wiki/Purposes_for_handling_Personal_Data#High-level_categories_.28to-be-discussed.29> ;
                          sw:term_status "accepted" .


###  http://w3.org/ns/dpv#Obtain
dpv:Obtain rdf:type owl:Class ;
           rdfs:subClassOf dpv:Processing ;
           dct:created "2019-04-04"^^xsd:date ;
           dct:date-accepted "2019-05-07"^^xsd:date ;
           dct:description "to solicit or gather data from someone"@en ;
           rdfs:isDefinedBy "DPVCG" ;
           sw:term_status "accepted" .


###  http://w3.org/ns/dpv#OfficialID
dpv:OfficialID rdf:type owl:Class ;
               rdfs:subClassOf dpv:Identifying ;
               dct:created "2019-04-04"^^xsd:date ;
               dct:creator "Elmar; Harshvardhan J. Pandit, Fajar" ;
               dct:date-accepted "2019-06-04"^^xsd:date ;
               dct:description "Information on an official identification document used by an individual."@en ;
               rdfs:isDefinedBy <https://enterprivacy.com/wp-content/uploads/2018/09/Categories-of-Personal-Information.pdf> ;
               rdfs:seeAlso svd:Government ;
               sw:term_status "accepted" .


###  http://w3.org/ns/dpv#Offspring
dpv:Offspring rdf:type owl:Class ;
              rdfs:subClassOf dpv:FamilyStructure ;
              dct:created "2019-04-04"^^xsd:date ;
              dct:creator "Elmar; Harshvardhan J. Pandit, Fajar" ;
              dct:date-accepted "2019-06-04"^^xsd:date ;
              dct:description "Information about an individual's offspring(s)."@en ;
              rdfs:isDefinedBy <https://enterprivacy.com/wp-content/uploads/2018/09/Categories-of-Personal-Information.pdf> ;
              sw:term_status "accepted" .


###  http://w3.org/ns/dpv#Opinion
dpv:Opinion rdf:type owl:Class ;
            rdfs:subClassOf dpv:Preference ;
            dct:created "2019-04-04"^^xsd:date ;
            dct:creator "Elmar; Harshvardhan J. Pandit, Fajar" ;
            dct:date-accepted "2019-06-04"^^xsd:date ;
            dct:description "Information about an individual's opinions"@en ;
            rdfs:isDefinedBy <https://enterprivacy.com/wp-content/uploads/2018/09/Categories-of-Personal-Information.pdf> ;
            sw:term_status "accepted" .


###  http://w3.org/ns/dpv#OptimisationForConsumer
dpv:OptimisationForConsumer rdf:type owl:Class ;
                            rdfs:subClassOf dpv:ServiceOptimization ;
                            dct:created "2018-12-10"^^xsd:date ;
                            dct:creator "Harshvardhan J. Pandit, Javier Fernandez, Axel Polleres, Elmar Kiesling, Fajar Ekaputra, Simon Steyskal" ;
                            dct:date-accepted "2019-04-05"^^xsd:date ;
                            dct:description "Optimisation of activities and services for the consumer or user"@en ;
                            rdfs:isDefinedBy <https://www.w3.org/community/dpvcg/wiki/Purposes_for_handling_Personal_Data#High-level_categories_.28to-be-discussed.29> ;
                            rdfs:seeAlso svpu:Custom ;
                            sw:term_status "accepted" .


###  http://w3.org/ns/dpv#OptimisationForController
dpv:OptimisationForController rdf:type owl:Class ;
                              rdfs:subClassOf dpv:ServiceOptimization ;
                              dct:created "2018-12-10"^^xsd:date ;
                              dct:creator "Harshvardhan J. Pandit, Javier Fernandez, Axel Polleres, Elmar Kiesling, Fajar Ekaputra, Simon Steyskal" ;
                              dct:date-accepted "2019-04-05"^^xsd:date ;
                              dct:description "Optimisation of activities and services for the Controller"@en ;
                              rdfs:isDefinedBy <https://www.w3.org/community/dpvcg/wiki/Purposes_for_handling_Personal_Data#High-level_categories_.28to-be-discussed.29> ;
                              sw:term_status "accepted" .


###  http://w3.org/ns/dpv#OptimiseUserInterface
dpv:OptimiseUserInterface rdf:type owl:Class ;
                          rdfs:subClassOf dpv:OptimisationForConsumer ;
                          dct:created "2018-12-10"^^xsd:date ;
                          dct:creator "Harshvardhan J. Pandit, Javier Fernandez, Axel Polleres, Elmar Kiesling, Fajar Ekaputra, Simon Steyskal" ;
                          dct:date-accepted "2019-04-05"^^xsd:date ;
                          dct:description "Optimisation of interfaces presented to the user"@en ;
                          rdfs:isDefinedBy <https://www.w3.org/community/dpvcg/wiki/Purposes_for_handling_Personal_Data#High-level_categories_.28to-be-discussed.29> ;
                          sw:term_status "accepted" .


###  http://w3.org/ns/dpv#OrganisationalMeasure
dpv:OrganisationalMeasure rdf:type owl:Class ;
                          rdfs:subClassOf dpv:TechnicalOrganisationalMeasure ;
                          dct:created "2019-04-04"^^xsd:date ;
                          dct:creator "Axel Polleres, Rob Brennan, Harshvardhan J. Pandit, Mark Lizar" ;
                          dct:date-accepted "2019-04-05"^^xsd:date ;
                          dct:description "Organisational measures required/followed when processing data of the declared category"@en ;
                          rdfs:isDefinedBy "DPVCG" ;
                          sw:term_status "accepted" .


###  http://w3.org/ns/dpv#Organise
dpv:Organise rdf:type owl:Class ;
             rdfs:subClassOf dpv:Organise ;
             dct:created "2019-04-04"^^xsd:date ;
             dct:date-accepted "2019-05-07"^^xsd:date ;
             dct:description "to organize data for arranging or classifying"@en ;
             rdfs:isDefinedBy <https://eur-lex.europa.eu/eli/reg/2016/679/art_4/par_2/oj> ;
             sw:term_status "accepted" .


###  http://w3.org/ns/dpv#Ownership
dpv:Ownership rdf:type owl:Class ;
              rdfs:subClassOf dpv:Financial ;
              dct:created "2019-04-04"^^xsd:date ;
              dct:creator "Elmar; Harshvardhan J. Pandit, Fajar" ;
              dct:date-accepted "2019-06-04"^^xsd:date ;
              dct:description "Information about things an individual has owned, rented, borrowed, possessed"@en ;
              rdfs:isDefinedBy <https://enterprivacy.com/wp-content/uploads/2018/09/Categories-of-Personal-Information.pdf> ;
              sw:term_status "accepted" .


###  http://w3.org/ns/dpv#PINCode
dpv:PINCode rdf:type owl:Class ;
            rdfs:subClassOf dpv:Authenticating ;
            dct:created "2019-04-04"^^xsd:date ;
            dct:creator "Elmar; Harshvardhan J. Pandit, Fajar" ;
            dct:date-accepted "2019-06-04"^^xsd:date ;
            dct:description "An individual's Personal identification number (PIN) used in the process of authenticating the individual as a user accessing a system."@en ;
            rdfs:isDefinedBy <https://enterprivacy.com/wp-content/uploads/2018/09/Categories-of-Personal-Information.pdf> ;
            sw:term_status "accepted" .


###  http://w3.org/ns/dpv#Parent
dpv:Parent rdf:type owl:Class ;
           rdfs:subClassOf dpv:FamilyStructure ;
           dct:created "2019-04-04"^^xsd:date ;
           dct:creator "Elmar; Harshvardhan J. Pandit, Fajar" ;
           dct:date-accepted "2019-06-04"^^xsd:date ;
           dct:description "Information about an individual's parent(s)."@en ;
           rdfs:isDefinedBy <https://enterprivacy.com/wp-content/uploads/2018/09/Categories-of-Personal-Information.pdf> ;
           sw:term_status "accepted" .


###  http://w3.org/ns/dpv#Password
dpv:Password rdf:type owl:Class ;
             rdfs:subClassOf dpv:Authenticating ;
             dct:created "2019-04-04"^^xsd:date ;
             dct:creator "Elmar; Harshvardhan J. Pandit, Fajar" ;
             dct:date-accepted "2019-06-04"^^xsd:date ;
             dct:description "An individual's password used in the process of authenticating the individual as a user accessing a system."@en ;
             rdfs:isDefinedBy <https://enterprivacy.com/wp-content/uploads/2018/09/Categories-of-Personal-Information.pdf> ;
             sw:term_status "accepted" .


###  http://w3.org/ns/dpv#PersonalDataCategory
dpv:PersonalDataCategory rdf:type owl:Class ;
                         dct:created "2019-04-04"^^xsd:date ;
                         dct:creator "Harshvardhan Pandit, Axel Polleres" ;
                         dct:date-accepted "2019-04-05"^^xsd:date ;
                         dct:description "A category of personal data (as defined by GDPR article 4.1) from the personal data categories taxonomy, i.e. for instance denoting the category of an object/field or data item that is used for processing"@en ;
                         rdfs:comment "Harsh: Change name to PersonalDataCategory since DataCategory can be non-personal data. Axel: Ageed" ;
                         rdfs:isDefinedBy <https://eur-lex.europa.eu/eli/reg/2016/679/art_4/par_1/pnt_g/oj> ,
                                          "DPVCG" ;
                         rdfs:seeAlso spl:AnyData ;
                         sw:term_status "accepted" .


###  http://w3.org/ns/dpv#PersonalDataHandling
dpv:PersonalDataHandling rdf:type owl:Class ;
                         dct:created "2019-04-04"^^xsd:date ;
                         dct:creator "Axel Polleres, Javier Ferenandez" ;
                         dct:date-accepted "2019-04-05"^^xsd:date ;
                         dct:description "Top Class to describe a concrete instance of legal personal Data Handling of a defined class of Data Subjects, meaning that a personal Data Category is undergoing specified processing by a specific data controller and/or transferred to some recipient for a particular purpose, based on a specific legal ground, with specified security measures and restrictions (e.g. storage locations and storage durations)."@en ;
                         sw:term_status "accepted" .


###  http://w3.org/ns/dpv#PersonalPossession
dpv:PersonalPossession rdf:type owl:Class ;
                       rdfs:subClassOf dpv:Ownership ;
                       dct:created "2019-04-04"^^xsd:date ;
                       dct:creator "Elmar; Harshvardhan J. Pandit, Fajar" ;
                       dct:date-accepted "2019-06-04"^^xsd:date ;
                       dct:description "Information about an individual's personal possessions."@en ;
                       rdfs:isDefinedBy <https://enterprivacy.com/wp-content/uploads/2018/09/Categories-of-Personal-Information.pdf> ;
                       sw:term_status "accepted" .


###  http://w3.org/ns/dpv#PersonalisedBenefits
dpv:PersonalisedBenefits rdf:type owl:Class ;
                         rdfs:subClassOf dpv:ServicePersonalization ;
                         dct:created "2018-12-10"^^xsd:date ;
                         dct:creator "Harshvardhan J. Pandit, Javier Fernandez, Axel Polleres, Elmar Kiesling, Fajar Ekaputra, Simon Steyskal" ;
                         dct:date-accepted "2019-04-05"^^xsd:date ;
                         dct:description "Personalisation of benefits received by the user"@en ;
                         rdfs:isDefinedBy <https://www.w3.org/community/dpvcg/wiki/Purposes_for_handling_Personal_Data#High-level_categories_.28to-be-discussed.29> ;
                         sw:term_status "accepted" .


###  http://w3.org/ns/dpv#Personality
dpv:Personality rdf:type owl:Class ;
                rdfs:subClassOf dpv:Behavioral ;
                dct:created "2019-04-04"^^xsd:date ;
                dct:creator "Elmar; Harshvardhan J. Pandit, Fajar" ;
                dct:date-accepted "2019-06-04"^^xsd:date ;
                dct:description "Information that relates to an individual's personality (e.g., categorization in terms of the Big Five personality traits)"@en ;
                rdfs:isDefinedBy <https://enterprivacy.com/wp-content/uploads/2018/09/Categories-of-Personal-Information.pdf> ;
                sw:term_status "accepted" .


###  http://w3.org/ns/dpv#PhilosophicalBelief
dpv:PhilosophicalBelief rdf:type owl:Class ;
                        rdfs:subClassOf dpv:KnowledgeBelief ,
                                        dpv:SpecialCategoryPersonalData ;
                        dct:created "2019-04-04"^^xsd:date ;
                        dct:creator "Elmar; Harshvardhan J. Pandit, Fajar" ;
                        dct:date-accepted "2019-06-04"^^xsd:date ;
                        dct:description "Information about an individual’s philosophical beliefs."@en ;
                        rdfs:isDefinedBy <https://enterprivacy.com/wp-content/uploads/2018/09/Categories-of-Personal-Information.pdf> ;
                        sw:term_status "accepted" .


###  http://w3.org/ns/dpv#PhysicalAddress
dpv:PhysicalAddress rdf:type owl:Class ;
                    rdfs:subClassOf dpv:Contact ;
                    dct:created "2019-04-04"^^xsd:date ;
                    dct:creator "Elmar; Harshvardhan J. Pandit, Fajar" ;
                    dct:date-accepted "2019-06-04"^^xsd:date ;
                    dct:description "Information about an individual's physical address."@en ;
                    rdfs:isDefinedBy <https://enterprivacy.com/wp-content/uploads/2018/09/Categories-of-Personal-Information.pdf> ;
                    sw:term_status "accepted" .


###  http://w3.org/ns/dpv#PhysicalCharacteristic
dpv:PhysicalCharacteristic rdf:type owl:Class ;
                           rdfs:subClassOf dpv:External ;
                           dct:created "2019-04-04"^^xsd:date ;
                           dct:creator "Elmar; Harshvardhan J. Pandit, Fajar" ;
                           dct:date-accepted "2019-06-04"^^xsd:date ;
                           dct:description "Information that describes an individual’s physical characteristics"@en ;
                           rdfs:isDefinedBy <https://enterprivacy.com/wp-content/uploads/2018/09/Categories-of-Personal-Information.pdf> ;
                           rdfs:seeAlso svd:Demographic ;
                           sw:term_status "accepted" .


###  http://w3.org/ns/dpv#PhysicalHealth
dpv:PhysicalHealth rdf:type owl:Class ;
                   rdfs:subClassOf dpv:Health ;
                   dct:created "2019-04-04"^^xsd:date ;
                   dct:creator "Elmar; Harshvardhan J. Pandit, Fajar" ;
                   dct:date-accepted "2019-06-04"^^xsd:date ;
                   dct:description "Information related to an individual's physical health."@en ;
                   rdfs:isDefinedBy <https://enterprivacy.com/wp-content/uploads/2018/09/Categories-of-Personal-Information.pdf> ;
                   sw:term_status "accepted" .


###  http://w3.org/ns/dpv#PhysicalTrait
dpv:PhysicalTrait rdf:type owl:Class ;
                  rdfs:subClassOf dpv:Demographic ;
                  dct:created "2019-04-04"^^xsd:date ;
                  dct:creator "Elmar; Harshvardhan J. Pandit, Fajar" ;
                  dct:date-accepted "2019-06-04"^^xsd:date ;
                  dct:description "Information on defining traits or features about an individuals body."@en ;
                  rdfs:isDefinedBy <https://enterprivacy.com/wp-content/uploads/2018/09/Categories-of-Personal-Information.pdf> ;
                  sw:term_status "accepted" .


###  http://w3.org/ns/dpv#Picture
dpv:Picture rdf:type owl:Class ;
            rdfs:subClassOf dpv:Identifying ;
            dct:created "2019-04-04"^^xsd:date ;
            dct:creator "Elmar; Harshvardhan J. Pandit, Fajar" ;
            dct:date-accepted "2019-06-04"^^xsd:date ;
            dct:description "A visual representation or image of an individual e.g. profile photo."@en ;
            rdfs:isDefinedBy <https://enterprivacy.com/wp-content/uploads/2018/09/Categories-of-Personal-Information.pdf> ;
            sw:term_status "accepted" .


###  http://w3.org/ns/dpv#Piercing
dpv:Piercing rdf:type owl:Class ;
             rdfs:subClassOf dpv:PhysicalCharacteristic ;
             dct:created "2019-04-04"^^xsd:date ;
             dct:creator "Elmar; Harshvardhan J. Pandit, Fajar" ;
             dct:date-accepted "2019-06-04"^^xsd:date ;
             dct:description "Information about an individual's piercings"@en ;
             rdfs:isDefinedBy <https://enterprivacy.com/wp-content/uploads/2018/09/Categories-of-Personal-Information.pdf> ;
             sw:term_status "accepted" .


###  http://w3.org/ns/dpv#PoliticalAffiliation
dpv:PoliticalAffiliation rdf:type owl:Class ;
                         rdfs:subClassOf dpv:PublicLife ,
                                         dpv:SpecialCategoryPersonalData ;
                         dct:created "2019-04-04"^^xsd:date ;
                         dct:creator "Elmar; Harshvardhan J. Pandit, Fajar" ;
                         dct:date-accepted "2019-06-04"^^xsd:date ;
                         dct:description "Information about an individual's political affiliation and history"@en ;
                         rdfs:isDefinedBy <https://enterprivacy.com/wp-content/uploads/2018/09/Categories-of-Personal-Information.pdf> ;
                         rdfs:seeAlso svd:Political ;
                         sw:term_status "accepted" .


###  http://w3.org/ns/dpv#Preference
dpv:Preference rdf:type owl:Class ;
               rdfs:subClassOf dpv:Internal ;
               dct:created "2019-04-04"^^xsd:date ;
               dct:creator "Elmar; Harshvardhan J. Pandit, Fajar" ;
               dct:date-accepted "2019-06-04"^^xsd:date ;
               dct:description "Information about an individual’s preferences or interests"@en ;
               rdfs:isDefinedBy <https://enterprivacy.com/wp-content/uploads/2018/09/Categories-of-Personal-Information.pdf> ;
               rdfs:seeAlso svd:Preference ;
               sw:term_status "accepted" .


###  http://w3.org/ns/dpv#Prescription
dpv:Prescription rdf:type owl:Class ;
                 rdfs:subClassOf dpv:MedicalHealth ;
                 dct:created "2019-04-04"^^xsd:date ;
                 dct:creator "Elmar; Harshvardhan J. Pandit, Fajar" ;
                 dct:date-accepted "2019-06-04"^^xsd:date ;
                 dct:description "Information about prescriptions made for an individual."@en ;
                 rdfs:isDefinedBy <https://enterprivacy.com/wp-content/uploads/2018/09/Categories-of-Personal-Information.pdf> ;
                 sw:term_status "accepted" .


###  http://w3.org/ns/dpv#PrivacyByDefault
dpv:PrivacyByDefault rdf:type owl:Class ;
                     rdfs:subClassOf dpv:GuidelinesPrinciple ;
                     dct:created "2019-04-04"^^xsd:date ;
                     dct:creator "Axel Polleres, Rob Brennan, Harshvardhan J. Pandit, Mark Lizar" ;
                     dct:date-accepted "2019-04-05"^^xsd:date ;
                     dct:description "Practices regarding selecting appropriate data protection and privacy measures as the 'default' in an activity or service"@en ;
                     rdfs:isDefinedBy "DPVCG" ;
                     sw:term_status "accepted" .


###  http://w3.org/ns/dpv#PrivacyByDesign
dpv:PrivacyByDesign rdf:type owl:Class ;
                    rdfs:subClassOf dpv:RiskManagementProcedure ;
                    dct:created "2019-04-04"^^xsd:date ;
                    dct:creator "Axel Polleres, Rob Brennan, Harshvardhan J. Pandit, Mark Lizar" ;
                    dct:date-accepted "2019-04-05"^^xsd:date ;
                    dct:description "Practices regarding incorporating data protection and privacy in the design of information and services"@en ;
                    rdfs:isDefinedBy "DPVCG" ;
                    sw:term_status "accepted" .


###  http://w3.org/ns/dpv#PrivacyPreference
dpv:PrivacyPreference rdf:type owl:Class ;
                      rdfs:subClassOf dpv:Preference ;
                      dct:created "2019-04-04"^^xsd:date ;
                      dct:creator "Elmar; Harshvardhan J. Pandit, Fajar" ;
                      dct:date-accepted "2019-06-04"^^xsd:date ;
                      dct:description "Information about an individual's privacy preferences"@en ;
                      rdfs:isDefinedBy <https://enterprivacy.com/wp-content/uploads/2018/09/Categories-of-Personal-Information.pdf> ;
                      sw:term_status "accepted" .


###  http://w3.org/ns/dpv#Processing
dpv:Processing rdf:type owl:Class ;
               dct:created "2019-04-04"^^xsd:date ;
               dct:creator "Axel Polleres, Javier Ferenandez" ;
               dct:date-accepted "2019-04-05"^^xsd:date ;
               dct:description "A type of processing from one of the processing categories in the processing Taxonomy"@en ;
               rdfs:isDefinedBy "DPVCG" ;
               rdfs:seeAlso spl:AnyProcessing ;
               sw:term_status "accepted" .


###  http://w3.org/ns/dpv#Proclivitie
dpv:Proclivitie rdf:type owl:Class ;
                rdfs:subClassOf dpv:Sexual ;
                dct:created "2019-04-04"^^xsd:date ;
                dct:creator "Elmar; Harshvardhan J. Pandit, Fajar" ;
                dct:date-accepted "2019-06-04"^^xsd:date ;
                dct:description "Information about an individual's proclivities in a sexual context"@en ;
                rdfs:isDefinedBy <https://enterprivacy.com/wp-content/uploads/2018/09/Categories-of-Personal-Information.pdf> ;
                sw:term_status "accepted" .


###  http://w3.org/ns/dpv#Professional
dpv:Professional rdf:type owl:Class ;
                 rdfs:subClassOf dpv:Social ;
                 dct:created "2019-04-04"^^xsd:date ;
                 dct:creator "Elmar; Harshvardhan J. Pandit, Fajar" ;
                 dct:date-accepted "2019-06-04"^^xsd:date ;
                 dct:description "Information about an individual’s educational or professional career"@en ;
                 rdfs:isDefinedBy <https://enterprivacy.com/wp-content/uploads/2018/09/Categories-of-Personal-Information.pdf> ;
                 sw:term_status "accepted" .


###  http://w3.org/ns/dpv#ProfessionalEvaluation
dpv:ProfessionalEvaluation rdf:type owl:Class ;
                           rdfs:subClassOf dpv:Professional ;
                           dct:created "2019-04-04"^^xsd:date ;
                           dct:creator "Elmar; Harshvardhan J. Pandit, Fajar" ;
                           dct:date-accepted "2019-06-04"^^xsd:date ;
                           dct:description "Information about professional evaluations associated with an individual"@en ;
                           rdfs:isDefinedBy <https://enterprivacy.com/wp-content/uploads/2018/09/Categories-of-Personal-Information.pdf> ;
                           sw:term_status "accepted" .


###  http://w3.org/ns/dpv#ProfessionalInterview
dpv:ProfessionalInterview rdf:type owl:Class ;
                          rdfs:subClassOf dpv:Professional ;
                          dct:created "2019-04-04"^^xsd:date ;
                          dct:creator "Elmar; Harshvardhan J. Pandit, Fajar" ;
                          dct:date-accepted "2019-06-04"^^xsd:date ;
                          dct:description "Information about professional interviews associated with an individual"@en ;
                          rdfs:isDefinedBy <https://enterprivacy.com/wp-content/uploads/2018/09/Categories-of-Personal-Information.pdf> ;
                          sw:term_status "accepted" .


###  http://w3.org/ns/dpv#Profiling
dpv:Profiling rdf:type owl:Class ;
              rdfs:subClassOf dpv:Use ;
              dct:created "2019-04-04"^^xsd:date ;
              dct:date-accepted "2019-05-07"^^xsd:date ;
              dct:description "to create a profile that describes or represents a person"@en ;
              rdfs:isDefinedBy "DPVCG" ;
              sw:term_status "accepted" .


###  http://w3.org/ns/dpv#PseudoAnonymise
dpv:PseudoAnonymise rdf:type owl:Class ;
                    rdfs:subClassOf dpv:Transform ;
                    dct:created "2019-04-04"^^xsd:date ;
                    dct:date-accepted "2019-05-07"^^xsd:date ;
                    dct:description "to replace personal identifiable information by artificial identifiers"@en ;
                    rdfs:isDefinedBy "DPVCG" ;
                    sw:term_status "accepted" .


###  http://w3.org/ns/dpv#PseudoAnonymization
dpv:PseudoAnonymization rdf:type owl:Class ;
                        rdfs:subClassOf dpv:PseudonymisationEncryption ;
                        dct:created "2019-04-04"^^xsd:date ;
                        dct:creator "Axel Polleres, Rob Brennan, Harshvardhan J. Pandit, Mark Lizar" ;
                        dct:date-accepted "2019-04-05"^^xsd:date ;
                        dct:description "PseudoAnonmyization or 'pseudonymisation’ means the processing of personal data in such a manner that the personal data can no longer be attributed to a specific data subject without the use of additional information, provided that such additional information is kept separately and is subject to technical and organisational measures to ensure that the personal data are not attributed to an identified or identifiable natural person;"@en ;
                        rdfs:isDefinedBy <https://eur-lex.europa.eu/eli/reg/2016/679/art_4/par_5/pnt_g/oj> ;
                        sw:term_status "accepted" .


###  http://w3.org/ns/dpv#PseudonymisationEncryption
dpv:PseudonymisationEncryption rdf:type owl:Class ;
                               rdfs:subClassOf dpv:TechnicalMeasure ;
                               dct:created "2019-04-04"^^xsd:date ;
                               dct:creator "Axel Polleres, Rob Brennan, Harshvardhan J. Pandit, Mark Lizar" ;
                               dct:date-accepted "2019-04-05"^^xsd:date ;
                               dct:description "Category of technical measures consisting of pseudoanonymization and encryption"@en ;
                               rdfs:isDefinedBy "DPVCG" ;
                               sw:term_status "accepted" .


###  http://w3.org/ns/dpv#PublicLife
dpv:PublicLife rdf:type owl:Class ;
               rdfs:subClassOf dpv:Social ;
               dct:created "2019-04-04"^^xsd:date ;
               dct:creator "Elmar; Harshvardhan J. Pandit, Fajar" ;
               dct:date-accepted "2019-06-04"^^xsd:date ;
               dct:description "Information about an individual’s public life"@en ;
               rdfs:isDefinedBy <https://enterprivacy.com/wp-content/uploads/2018/09/Categories-of-Personal-Information.pdf> ;
               sw:term_status "accepted" .


###  http://w3.org/ns/dpv#Purchase
dpv:Purchase rdf:type owl:Class ;
             rdfs:subClassOf dpv:Transactional ;
             dct:created "2019-04-04"^^xsd:date ;
             dct:creator "Elmar; Harshvardhan J. Pandit, Fajar" ;
             dct:date-accepted "2019-06-04"^^xsd:date ;
             dct:description "Information about purchases such as items bought e.g. grocery or clothing"@en ;
             rdfs:isDefinedBy <https://enterprivacy.com/wp-content/uploads/2018/09/Categories-of-Personal-Information.pdf> ;
             rdfs:seeAlso svd:Purchase ;
             sw:term_status "accepted" .


###  http://w3.org/ns/dpv#PurchasesAndSpendingHabit
dpv:PurchasesAndSpendingHabit rdf:type owl:Class ;
                              rdfs:subClassOf dpv:Transactional ;
                              dct:created "2019-04-04"^^xsd:date ;
                              dct:creator "Elmar; Harshvardhan J. Pandit, Fajar" ;
                              dct:date-accepted "2019-06-04"^^xsd:date ;
                              dct:description "Information about analysis of purchases made and money spent expressed as a habit e.g. monthly shopping trends"@en ;
                              rdfs:isDefinedBy <https://enterprivacy.com/wp-content/uploads/2018/09/Categories-of-Personal-Information.pdf> ;
                              sw:term_status "accepted" .


###  http://w3.org/ns/dpv#Purpose
dpv:Purpose rdf:type owl:Class ;
            dct:created "2019-04-04"^^xsd:date ;
            dct:creator "Axel Polleres, Javier Ferenandez" ;
            dct:date-accepted "2019-04-05"^^xsd:date ;
            dct:description "The purpose of Data Handling, from the purposes Taxonomy"@en ;
            rdfs:isDefinedBy "DPVCG" ;
            rdfs:seeAlso spl:AnyPurpose ;
            sw:term_status "accepted" .


###  http://w3.org/ns/dpv#Race
dpv:Race rdf:type owl:Class ;
         rdfs:subClassOf dpv:Ethnicity ,
                         dpv:SpecialCategoryPersonalData ;
         dct:created "2019-04-04"^^xsd:date ;
         dct:creator "Elmar; Harshvardhan J. Pandit, Fajar" ;
         dct:date-accepted "2019-06-04"^^xsd:date ;
         dct:description "Information related to an individual's race."@en ;
         rdfs:isDefinedBy <https://enterprivacy.com/wp-content/uploads/2018/09/Categories-of-Personal-Information.pdf> ;
         sw:term_status "accepted" .


###  http://w3.org/ns/dpv#Recipient
dpv:Recipient rdf:type owl:Class ;
              dct:created "2019-04-04"^^xsd:date ;
              dct:creator "Axel Polleres, Javier Ferenandez" ;
              dct:date-accepted "2019-04-05"^^xsd:date ;
              dct:description "The entities that can access the result of a data handling action/processing, any legal entity that is defined by article 4.9 of GDPR, which states - 'recipient' means a natural or legal person, public authority, agency or another body, to which the personal data are disclosed, whether a third party or not."@en ;
              rdfs:isDefinedBy <https://eur-lex.europa.eu/eli/reg/2016/679/art_4/par_9/pnt_g/oj> ,
                               "DPVCG" ;
              rdfs:seeAlso spl:AnyRecipient ;
              sw:term_status "accepted" .


###  http://w3.org/ns/dpv#Record
dpv:Record rdf:type owl:Class ;
           rdfs:subClassOf dpv:Obtain ;
           dct:created "2019-04-04"^^xsd:date ;
           dct:date-accepted "2019-05-07"^^xsd:date ;
           dct:description "to make a record (especially media)"@en ;
           rdfs:isDefinedBy <https://eur-lex.europa.eu/eli/reg/2016/679/art_4/par_2/oj> ;
           sw:term_status "accepted" .


###  http://w3.org/ns/dpv#Reference
dpv:Reference rdf:type owl:Class ;
              rdfs:subClassOf dpv:Professional ;
              dct:created "2019-04-04"^^xsd:date ;
              dct:creator "Elmar; Harshvardhan J. Pandit, Fajar" ;
              dct:date-accepted "2019-06-04"^^xsd:date ;
              dct:description "Information about an individual's references in the professional context"@en ;
              rdfs:isDefinedBy <https://enterprivacy.com/wp-content/uploads/2018/09/Categories-of-Personal-Information.pdf> ;
              sw:term_status "accepted" .


###  http://w3.org/ns/dpv#RegularityOfRecertification
dpv:RegularityOfRecertification rdf:type owl:Class ;
                                rdfs:subClassOf dpv:RiskManagementProcedure ;
                                dct:created "2019-04-04"^^xsd:date ;
                                dct:creator "Axel Polleres, Rob Brennan, Harshvardhan J. Pandit, Mark Lizar" ;
                                dct:date-accepted "2019-04-05"^^xsd:date ;
                                dct:description "Specifies policy regarding repetition or renewal of existing certification(s)"@en ;
                                rdfs:isDefinedBy "DPVCG" ;
                                sw:term_status "accepted" .


###  http://w3.org/ns/dpv#Relationship
dpv:Relationship rdf:type owl:Class ;
                 rdfs:subClassOf dpv:Family ;
                 dct:created "2019-04-04"^^xsd:date ;
                 dct:creator "Elmar; Harshvardhan J. Pandit, Fajar" ;
                 dct:date-accepted "2019-06-04"^^xsd:date ;
                 dct:description "Information that characterizes an individual's relationships with other individuals."@en ;
                 rdfs:isDefinedBy <https://enterprivacy.com/wp-content/uploads/2018/09/Categories-of-Personal-Information.pdf> ;
                 sw:term_status "accepted" .


###  http://w3.org/ns/dpv#Religion
dpv:Religion rdf:type owl:Class ;
             rdfs:subClassOf dpv:PublicLife ,
                             dpv:SpecialCategoryPersonalData ;
             dct:created "2019-04-04"^^xsd:date ;
             dct:creator "Elmar; Harshvardhan J. Pandit, Fajar" ;
             dct:date-accepted "2019-06-04"^^xsd:date ;
             dct:description "Information about an individual's religion, religious inclinations, and religious history."@en ;
             rdfs:isDefinedBy <https://enterprivacy.com/wp-content/uploads/2018/09/Categories-of-Personal-Information.pdf> ;
             sw:term_status "accepted" .


###  http://w3.org/ns/dpv#ReligiousBelief
dpv:ReligiousBelief rdf:type owl:Class ;
                    rdfs:subClassOf dpv:KnowledgeBelief ,
                                    dpv:SpecialCategoryPersonalData ;
                    dct:created "2019-04-04"^^xsd:date ;
                    dct:creator "Elmar; Harshvardhan J. Pandit, Fajar" ;
                    dct:date-accepted "2019-06-04"^^xsd:date ;
                    dct:description "Information about an individual’s religious beliefs."@en ;
                    rdfs:isDefinedBy <https://enterprivacy.com/wp-content/uploads/2018/09/Categories-of-Personal-Information.pdf> ;
                    sw:term_status "accepted" .


###  http://w3.org/ns/dpv#Remove
dpv:Remove rdf:type owl:Class ;
           rdfs:subClassOf dpv:Processing ;
           dct:created "2019-04-04"^^xsd:date ;
           dct:date-accepted "2019-05-07"^^xsd:date ;
           dct:description "to destruct or erase data"@en ;
           rdfs:isDefinedBy "DPVCG" ;
           sw:term_status "accepted" .


###  http://w3.org/ns/dpv#ResearchAndDevelopment
dpv:ResearchAndDevelopment rdf:type owl:Class ;
                           rdfs:subClassOf dpv:Purpose ;
                           dct:created "2018-12-10"^^xsd:date ;
                           dct:creator "Harshvardhan J. Pandit, Javier Fernandez, Axel Polleres, Elmar Kiesling, Fajar Ekaputra, Simon Steyskal" ;
                           dct:date-accepted "2019-04-05"^^xsd:date ;
                           dct:description "Performing research and developing new methods,products, or services"@en ;
                           rdfs:isDefinedBy <https://www.w3.org/community/dpvcg/wiki/Purposes_for_handling_Personal_Data#High-level_categories_.28to-be-discussed.29> ;
                           sw:term_status "accepted" .


###  http://w3.org/ns/dpv#Restrict
dpv:Restrict rdf:type owl:Class ;
             rdfs:subClassOf dpv:Transform ;
             dct:created "2019-04-04"^^xsd:date ;
             dct:date-accepted "2019-05-07"^^xsd:date ;
             dct:description "to apply a restriction on the processsing of specific records"@en ;
             rdfs:isDefinedBy <https://eur-lex.europa.eu/eli/reg/2016/679/art_4/par_2/oj> ;
             sw:term_status "accepted" .


###  http://w3.org/ns/dpv#Retina
dpv:Retina rdf:type owl:Class ;
           rdfs:subClassOf dpv:Biometric ;
           dct:created "2019-04-04"^^xsd:date ;
           dct:creator "Elmar; Harshvardhan J. Pandit, Fajar" ;
           dct:date-accepted "2019-06-04"^^xsd:date ;
           dct:description "Information related to an individual's retina used for biometric purposes."@en ;
           rdfs:isDefinedBy <https://enterprivacy.com/wp-content/uploads/2018/09/Categories-of-Personal-Information.pdf> ;
           sw:term_status "accepted" .


###  http://w3.org/ns/dpv#Retrieve
dpv:Retrieve rdf:type owl:Class ;
             rdfs:subClassOf dpv:Use ;
             dct:created "2019-04-04"^^xsd:date ;
             dct:date-accepted "2019-05-07"^^xsd:date ;
             dct:description "to retrieve data, often in an automated manner"@en ;
             rdfs:isDefinedBy <https://eur-lex.europa.eu/eli/reg/2016/679/art_4/par_2/oj> ;
             sw:term_status "accepted" .


###  http://w3.org/ns/dpv#RiskManagementProcedure
dpv:RiskManagementProcedure rdf:type owl:Class ;
                            rdfs:subClassOf dpv:OrganisationalMeasure ;
                            dct:created "2019-04-04"^^xsd:date ;
                            dct:creator "Axel Polleres, Rob Brennan, Harshvardhan J. Pandit, Mark Lizar" ;
                            dct:date-accepted "2019-04-05"^^xsd:date ;
                            dct:description "Risk management refers to a coordinated set of activities and methods that is used to direct an organization and to control the many risks that can affect its ability to achieve objectives.  The term risk management also refers to the programme that is used to manage risk. This programme includes risk management principles, a risk management framework, and a risk management process."@en ;
                            rdfs:comment "Data Protection Impact Assessments as per GDPR art 35, other Privacy Impact Assessments, threat severity assessment https://www.cnil.fr/en/privacy-impact-assessment-pia" ;
                            rdfs:isDefinedBy "DPVCG" ;
                            sw:term_status "accepted" .


###  http://w3.org/ns/dpv#RoomNumber
dpv:RoomNumber rdf:type owl:Class ;
               rdfs:subClassOf dpv:Location ;
               dct:created "2019-04-04"^^xsd:date ;
               dct:creator "Elmar; Harshvardhan J. Pandit, Fajar" ;
               dct:date-accepted "2019-06-04"^^xsd:date ;
               dct:description "Room number of a location associated with an individual."@en ;
               rdfs:isDefinedBy <https://enterprivacy.com/wp-content/uploads/2018/09/Categories-of-Personal-Information.pdf> ;
               sw:term_status "accepted" .


###  http://w3.org/ns/dpv#Salary
dpv:Salary rdf:type owl:Class ;
           rdfs:subClassOf dpv:Professional ;
           dct:created "2019-04-04"^^xsd:date ;
           dct:creator "Elmar; Harshvardhan J. Pandit, Fajar" ;
           dct:date-accepted "2019-06-04"^^xsd:date ;
           dct:description "Information about an individual's salary"@en ;
           rdfs:isDefinedBy <https://enterprivacy.com/wp-content/uploads/2018/09/Categories-of-Personal-Information.pdf> ;
           sw:term_status "accepted" .


###  http://w3.org/ns/dpv#Sale
dpv:Sale rdf:type owl:Class ;
         rdfs:subClassOf dpv:Transactional ;
         dct:created "2019-04-04"^^xsd:date ;
         dct:creator "Elmar; Harshvardhan J. Pandit, Fajar" ;
         dct:date-accepted "2019-06-04"^^xsd:date ;
         dct:description "Information about sales e.g. selling of goods or services"@en ;
         rdfs:isDefinedBy <https://enterprivacy.com/wp-content/uploads/2018/09/Categories-of-Personal-Information.pdf> ;
         sw:term_status "accepted" .


###  http://w3.org/ns/dpv#School
dpv:School rdf:type owl:Class ;
           rdfs:subClassOf dpv:Professional ;
           dct:created "2019-04-04"^^xsd:date ;
           dct:creator "Elmar; Harshvardhan J. Pandit, Fajar" ;
           dct:date-accepted "2019-06-04"^^xsd:date ;
           dct:description "Information about an individual's school such as name of school, conduct, or grades obtained."@en ;
           rdfs:isDefinedBy <https://enterprivacy.com/wp-content/uploads/2018/09/Categories-of-Personal-Information.pdf> ;
           sw:term_status "accepted" .


###  http://w3.org/ns/dpv#Seal
dpv:Seal rdf:type owl:Class ;
         rdfs:subClassOf dpv:CertificationSeal ;
         dct:created "2019-04-04"^^xsd:date ;
         dct:creator "Axel Polleres, Rob Brennan, Harshvardhan J. Pandit, Mark Lizar" ;
         dct:date-accepted "2019-04-05"^^xsd:date ;
         dct:description "a seal or a mark indicating proof of certification to some certification or standard"@en ;
         rdfs:isDefinedBy "DPVCG" ;
         sw:term_status "accepted" .


###  http://w3.org/ns/dpv#SecretText
dpv:SecretText rdf:type owl:Class ;
               rdfs:subClassOf dpv:Authenticating ;
               dct:created "2019-04-04"^^xsd:date ;
               dct:creator "Elmar; Harshvardhan J. Pandit, Fajar" ;
               dct:date-accepted "2019-06-04"^^xsd:date ;
               dct:description "An individual's secret text used in the process of authenticating the individual as a user accessing a system, e.g., when recovering a lost password."@en ;
               rdfs:isDefinedBy <https://enterprivacy.com/wp-content/uploads/2018/09/Categories-of-Personal-Information.pdf> ;
               sw:term_status "accepted" .


###  http://w3.org/ns/dpv#Sector
dpv:Sector rdf:type owl:Class ;
           dct:created "2019-04-04"^^xsd:date ;
           dct:date-accepted "2019-04-05"^^xsd:date ;
           dct:description "Used to indicate the sector of a purpose e.g. Agriculture, Advertising (specified e.g. in the form of NACE codes)"@en ;
           sw:term_status "accepted" .


###  http://w3.org/ns/dpv#Security
dpv:Security rdf:type owl:Class ;
             rdfs:subClassOf dpv:Purpose ;
             dct:created "2018-12-10"^^xsd:date ;
             dct:creator "Harshvardhan J. Pandit, Javier Fernandez, Axel Polleres, Elmar Kiesling, Fajar Ekaputra, Simon Steyskal" ;
             dct:date-accepted "2019-04-05"^^xsd:date ;
             dct:description "Security of data"@en ;
             rdfs:isDefinedBy <https://www.w3.org/community/dpvcg/wiki/Purposes_for_handling_Personal_Data#High-level_categories_.28to-be-discussed.29> ;
             sw:term_status "accepted" .


###  http://w3.org/ns/dpv#SellDataToThirdParties
dpv:SellDataToThirdParties rdf:type owl:Class ;
                           rdfs:subClassOf dpv:CommercialInterest ;
                           dct:created "2018-12-10"^^xsd:date ;
                           dct:creator "Harshvardhan J. Pandit, Javier Fernandez, Axel Polleres, Elmar Kiesling, Fajar Ekaputra, Simon Steyskal" ;
                           dct:date-accepted "2019-04-05"^^xsd:date ;
                           dct:description "To sell data or information to third parties"@en ;
                           rdfs:isDefinedBy <https://www.w3.org/community/dpvcg/wiki/Purposes_for_handling_Personal_Data#High-level_categories_.28to-be-discussed.29> ;
                           sw:term_status "accepted" .


###  http://w3.org/ns/dpv#SellInsightsFromData
dpv:SellInsightsFromData rdf:type owl:Class ;
                         rdfs:subClassOf dpv:CommercialInterest ;
                         dct:created "2018-12-10"^^xsd:date ;
                         dct:creator "Harshvardhan J. Pandit, Javier Fernandez, Axel Polleres, Elmar Kiesling, Fajar Ekaputra, Simon Steyskal" ;
                         dct:date-accepted "2019-04-05"^^xsd:date ;
                         dct:description "To sell or commercially provide insights obtained from analysis of data"@en ;
                         rdfs:isDefinedBy <https://www.w3.org/community/dpvcg/wiki/Purposes_for_handling_Personal_Data#High-level_categories_.28to-be-discussed.29> ;
                         sw:term_status "accepted" .


###  http://w3.org/ns/dpv#SellProductsToDataSubject
dpv:SellProductsToDataSubject rdf:type owl:Class ;
                              rdfs:subClassOf dpv:CommercialInterest ;
                              dct:created "2018-12-10"^^xsd:date ;
                              dct:creator "Harshvardhan J. Pandit, Javier Fernandez, Axel Polleres, Elmar Kiesling, Fajar Ekaputra, Simon Steyskal" ;
                              dct:date-accepted "2019-04-05"^^xsd:date ;
                              dct:description "To sell products or services to the data subject or user"@en ;
                              rdfs:isDefinedBy <https://www.w3.org/community/dpvcg/wiki/Purposes_for_handling_Personal_Data#High-level_categories_.28to-be-discussed.29> ;
                              sw:term_status "accepted" .


###  http://w3.org/ns/dpv#SellTargettedAdvertisements
dpv:SellTargettedAdvertisements rdf:type owl:Class ;
                                rdfs:subClassOf dpv:CommercialInterest ;
                                dct:created "2018-12-10"^^xsd:date ;
                                dct:creator "Harshvardhan J. Pandit, Javier Fernandez, Axel Polleres, Elmar Kiesling, Fajar Ekaputra, Simon Steyskal" ;
                                dct:date-accepted "2019-04-05"^^xsd:date ;
                                dct:description "To sell or provide targetted advertisements about the user to Third Parties"@en ;
                                rdfs:isDefinedBy <https://www.w3.org/community/dpvcg/wiki/Purposes_for_handling_Personal_Data#High-level_categories_.28to-be-discussed.29> ;
                                sw:term_status "accepted" .


###  http://w3.org/ns/dpv#ServiceConsumptionBehavior
dpv:ServiceConsumptionBehavior rdf:type owl:Class ;
                               rdfs:subClassOf dpv:ServicePersonalization ;
                               dct:created "2019-11-25"^^xsd:date ;
                               dct:creator "Harshvardhan J. Pandit, Rudy Jacob" ;
                               dct:description "Information about the consumption of a service by an individual. Examples: time and duration of consumption."@en ;
                               sw:term_status "proposed" .


###  http://w3.org/ns/dpv#ServiceOptimization
dpv:ServiceOptimization rdf:type owl:Class ;
                        rdfs:subClassOf dpv:Purpose ;
                        dct:created "2018-12-10"^^xsd:date ;
                        dct:creator "Harshvardhan J. Pandit, Javier Fernandez, Axel Polleres, Elmar Kiesling, Fajar Ekaputra, Simon Steyskal" ;
                        dct:date-accepted "2019-04-05"^^xsd:date ;
                        dct:description "Optimization of service or activity"@en ;
                        rdfs:isDefinedBy <https://www.w3.org/community/dpvcg/wiki/Purposes_for_handling_Personal_Data#High-level_categories_.28to-be-discussed.29> ;
                        sw:term_status "accepted" .


###  http://w3.org/ns/dpv#ServicePersonalization
dpv:ServicePersonalization rdf:type owl:Class ;
                           rdfs:subClassOf dpv:Purpose ;
                           dct:created "2018-12-10"^^xsd:date ;
                           dct:creator "Harshvardhan J. Pandit, Javier Fernandez, Axel Polleres, Elmar Kiesling, Fajar Ekaputra, Simon Steyskal" ;
                           dct:date-accepted "2019-04-05"^^xsd:date ;
                           dct:description "Personalization of service or activity for the user"@en ;
                           rdfs:isDefinedBy <https://www.w3.org/community/dpvcg/wiki/Purposes_for_handling_Personal_Data#High-level_categories_.28to-be-discussed.29> ;
                           sw:term_status "accepted" .


###  http://w3.org/ns/dpv#ServiceProvision
dpv:ServiceProvision rdf:type owl:Class ;
                     rdfs:subClassOf dpv:Purpose ;
                     dct:created "2018-12-10"^^xsd:date ;
                     dct:creator "Harshvardhan J. Pandit, Javier Fernandez, Axel Polleres, Elmar Kiesling, Fajar Ekaputra, Simon Steyskal" ;
                     dct:date-accepted "2019-04-05"^^xsd:date ;
                     dct:description "Provision of service or activity"@en ;
                     rdfs:isDefinedBy <https://www.w3.org/community/dpvcg/wiki/Purposes_for_handling_Personal_Data#High-level_categories_.28to-be-discussed.29> ;
                     sw:term_status "accepted" .


###  http://w3.org/ns/dpv#Sexual
dpv:Sexual rdf:type owl:Class ;
           rdfs:subClassOf dpv:External ,
                           dpv:SpecialCategoryPersonalData ;
           dct:created "2019-04-04"^^xsd:date ;
           dct:creator "Elmar; Harshvardhan J. Pandit, Fajar" ;
           dct:date-accepted "2019-06-04"^^xsd:date ;
           dct:description "Information that describes an individual’s sexual life"@en ;
           rdfs:isDefinedBy <https://enterprivacy.com/wp-content/uploads/2018/09/Categories-of-Personal-Information.pdf> ;
           sw:term_status "accepted" .


###  http://w3.org/ns/dpv#SexualHistory
dpv:SexualHistory rdf:type owl:Class ;
                  rdfs:subClassOf dpv:Sexual ;
                  dct:created "2019-04-04"^^xsd:date ;
                  dct:creator "Elmar; Harshvardhan J. Pandit, Fajar" ;
                  dct:date-accepted "2019-06-04"^^xsd:date ;
                  dct:description "Information about an individual's sexual history"@en ;
                  rdfs:isDefinedBy <https://enterprivacy.com/wp-content/uploads/2018/09/Categories-of-Personal-Information.pdf> ;
                  sw:term_status "accepted" .


###  http://w3.org/ns/dpv#SexualPreference
dpv:SexualPreference rdf:type owl:Class ;
                     rdfs:subClassOf dpv:Sexual ;
                     dct:created "2019-04-04"^^xsd:date ;
                     dct:creator "Elmar; Harshvardhan J. Pandit, Fajar" ;
                     dct:date-accepted "2019-06-04"^^xsd:date ;
                     dct:description "Information about an individual's sexual preferences"@en ;
                     rdfs:isDefinedBy <https://enterprivacy.com/wp-content/uploads/2018/09/Categories-of-Personal-Information.pdf> ;
                     sw:term_status "accepted" .


###  http://w3.org/ns/dpv#Share
dpv:Share rdf:type owl:Class ;
          rdfs:subClassOf dpv:Disclose ;
          dct:created "2019-04-04"^^xsd:date ;
          dct:date-accepted "2019-05-07"^^xsd:date ;
          dct:description "to give data (or a portion of it) to others"@en ;
          rdfs:isDefinedBy "DPVCG" ;
          sw:term_status "accepted" .


###  http://w3.org/ns/dpv#Sibling
dpv:Sibling rdf:type owl:Class ;
            rdfs:subClassOf dpv:FamilyStructure ;
            dct:created "2019-04-04"^^xsd:date ;
            dct:creator "Elmar; Harshvardhan J. Pandit, Fajar" ;
            dct:date-accepted "2019-06-04"^^xsd:date ;
            dct:description "Information about an individual's sibling(s)."@en ;
            rdfs:isDefinedBy <https://enterprivacy.com/wp-content/uploads/2018/09/Categories-of-Personal-Information.pdf> ;
            sw:term_status "accepted" .


###  http://w3.org/ns/dpv#SkinTone
dpv:SkinTone rdf:type owl:Class ;
             rdfs:subClassOf dpv:PhysicalCharacteristic ;
             dct:created "2019-04-04"^^xsd:date ;
             dct:creator "Elmar; Harshvardhan J. Pandit, Fajar" ;
             dct:date-accepted "2019-06-04"^^xsd:date ;
             dct:description "Information about an individual's skin tone"@en ;
             rdfs:isDefinedBy <https://enterprivacy.com/wp-content/uploads/2018/09/Categories-of-Personal-Information.pdf> ;
             sw:term_status "accepted" .


###  http://w3.org/ns/dpv#Social
dpv:Social rdf:type owl:Class ;
           rdfs:subClassOf dpv:PersonalDataCategory ;
           dct:created "2019-04-04"^^xsd:date ;
           dct:creator "Elmar; Harshvardhan J. Pandit, Fajar" ;
           dct:date-accepted "2019-06-04"^^xsd:date ;
           dct:description "Personal data about the social aspects such as for family, public life, or professional networks."@en ;
           rdfs:isDefinedBy <https://enterprivacy.com/wp-content/uploads/2018/09/Categories-of-Personal-Information.pdf> ;
           sw:term_status "accepted" .


###  http://w3.org/ns/dpv#SocialMediaCommunication
dpv:SocialMediaCommunication rdf:type owl:Class ;
                             rdfs:subClassOf dpv:Communication ;
                             dct:created "2019-04-04"^^xsd:date ;
                             dct:creator "Elmar; Harshvardhan J. Pandit, Fajar" ;
                             dct:date-accepted "2019-06-04"^^xsd:date ;
                             dct:description "Information relating to an individual's social media communication, including the communication itself and metadata."@en ;
                             rdfs:isDefinedBy <https://enterprivacy.com/wp-content/uploads/2018/09/Categories-of-Personal-Information.pdf> ;
                             rdfs:seeAlso svd:Social ;
                             sw:term_status "accepted" .


###  http://w3.org/ns/dpv#SocialNetwork
dpv:SocialNetwork rdf:type owl:Class ;
                  rdfs:subClassOf dpv:Social ;
                  dct:created "2019-04-04"^^xsd:date ;
                  dct:creator "Elmar; Harshvardhan J. Pandit, Fajar" ;
                  dct:date-accepted "2019-06-04"^^xsd:date ;
                  dct:description "Information about an individual’s friends or connections expressed as a social network"@en ;
                  rdfs:isDefinedBy <https://enterprivacy.com/wp-content/uploads/2018/09/Categories-of-Personal-Information.pdf> ;
                  sw:term_status "accepted" .


###  http://w3.org/ns/dpv#SocialStatus
dpv:SocialStatus rdf:type owl:Class ;
                 rdfs:subClassOf dpv:PublicLife ;
                 dct:created "2019-04-04"^^xsd:date ;
                 dct:creator "Elmar; Harshvardhan J. Pandit, Fajar" ;
                 dct:date-accepted "2019-06-04"^^xsd:date ;
                 dct:description "Information about an individual's social status"@en ;
                 rdfs:isDefinedBy <https://enterprivacy.com/wp-content/uploads/2018/09/Categories-of-Personal-Information.pdf> ;
                 sw:term_status "accepted" .


###  http://w3.org/ns/dpv#SpecialCategoryPersonalData
dpv:SpecialCategoryPersonalData rdf:type owl:Class ;
                                rdfs:subClassOf dpv:PersonalDataCategory ;
                                dct:created "2019-04-04"^^xsd:date ;
                                dct:creator "Elmar; Harshvardhan J. Pandit, Fajar" ;
                                dct:date-accepted "2019-05-07"^^xsd:date ;
                                dct:description "Special category or personal data as per GDPR Art. 9 (1)"@en ;
                                rdfs:isDefinedBy <https://eur-lex.europa.eu/eli/reg/2016/679/art_9/par_1/oj> ;
                                sw:term_status "accepted" .


###  http://w3.org/ns/dpv#StaffTraining
dpv:StaffTraining rdf:type owl:Class ;
                  rdfs:subClassOf dpv:RiskManagementProcedure ;
                  dct:created "2019-04-04"^^xsd:date ;
                  dct:creator "Axel Polleres, Rob Brennan, Harshvardhan J. Pandit, Mark Lizar" ;
                  dct:date-accepted "2019-04-05"^^xsd:date ;
                  dct:description "Practices and policies regarding training of staff members"@en ;
                  rdfs:isDefinedBy "DPVCG" ;
                  sw:term_status "accepted" .


###  http://w3.org/ns/dpv#StorageDeletion
dpv:StorageDeletion rdf:type owl:Class ;
                    rdfs:subClassOf dpv:StorageRestriction ;
                    dct:created "2019-04-04"^^xsd:date ;
                    dct:creator "Axel Polleres, Rob Brennan, Harshvardhan J. Pandit, Mark Lizar" ;
                    dct:date-accepted "2019-04-05"^^xsd:date ;
                    dct:description "Defines how secure deletion is guaranteed"@en ;
                    rdfs:isDefinedBy "DPVCG" ;
                    sw:term_status "accepted" .


###  http://w3.org/ns/dpv#StorageDuration
dpv:StorageDuration rdf:type owl:Class ;
                    rdfs:subClassOf dpv:StorageRestriction ;
                    dct:created "2019-04-04"^^xsd:date ;
                    dct:creator "Axel Polleres, Rob Brennan, Harshvardhan J. Pandit, Mark Lizar" ;
                    dct:date-accepted "2019-04-05"^^xsd:date ;
                    dct:description "A duration or temporal entity denoting limitation on storage of personal data"@en ;
                    rdfs:isDefinedBy "DPVCG" ;
                    sw:term_status "accepted" .


###  http://w3.org/ns/dpv#StorageLocation
dpv:StorageLocation rdf:type owl:Class ;
                    rdfs:subClassOf dpv:StorageRestriction ;
                    dct:created "2019-04-04"^^xsd:date ;
                    dct:creator "Axel Polleres, Rob Brennan, Harshvardhan J. Pandit, Mark Lizar" ;
                    dct:date-accepted "2019-04-05"^^xsd:date ;
                    dct:description "Defines a location or goespatial scope, where the data is (physically) stored"@en ;
                    rdfs:isDefinedBy "DPVCG" ;
                    sw:term_status "accepted" .


###  http://w3.org/ns/dpv#StorageRestoration
dpv:StorageRestoration rdf:type owl:Class ;
                       rdfs:subClassOf dpv:StorageRestriction ;
                       dct:created "2019-04-04"^^xsd:date ;
                       dct:creator "Axel Polleres, Rob Brennan, Harshvardhan J. Pandit, Mark Lizar" ;
                       dct:date-accepted "2019-04-05"^^xsd:date ;
                       dct:description "Regularity and temporal span of data restoration/backup mechanisms that guarantee that data is preserved"@en ;
                       rdfs:isDefinedBy "DPVCG" ;
                       sw:term_status "accepted" .


###  http://w3.org/ns/dpv#StorageRestriction
dpv:StorageRestriction rdf:type owl:Class ;
                       rdfs:subClassOf dpv:TechnicalMeasure ;
                       dct:created "2019-04-04"^^xsd:date ;
                       dct:creator "Axel Polleres, Rob Brennan, Harshvardhan J. Pandit, Mark Lizar" ;
                       dct:date-accepted "2019-04-05"^^xsd:date ;
                       dct:description "Restrictions required or followed regarding storage of data"@en ;
                       rdfs:isDefinedBy "DPVCG" ;
                       sw:term_status "accepted" .


###  http://w3.org/ns/dpv#Store
dpv:Store rdf:type owl:Class ;
          rdfs:subClassOf dpv:Processing ;
          dct:created "2019-04-04"^^xsd:date ;
          dct:date-accepted "2019-05-07"^^xsd:date ;
          dct:description "to keep data for future use"@en ;
          rdfs:isDefinedBy <https://eur-lex.europa.eu/eli/reg/2016/679/art_4/par_2/oj> ;
          sw:term_status "accepted" .


###  http://w3.org/ns/dpv#Structure
dpv:Structure rdf:type owl:Class ;
              rdfs:subClassOf dpv:Organise ;
              dct:created "2019-04-04"^^xsd:date ;
              dct:date-accepted "2019-05-07"^^xsd:date ;
              dct:description "to arrange data according to a structure"@en ;
              rdfs:isDefinedBy <https://eur-lex.europa.eu/eli/reg/2016/679/art_4/par_2/oj> ;
              sw:term_status "accepted" .


###  http://w3.org/ns/dpv#TVViewingBehavior
dpv:TVViewingBehavior rdf:type owl:Class ;
                      rdfs:subClassOf dpv:ServiceConsumptionBehavior ;
                      dct:created "2019-11-25"^^xsd:date ;
                      dct:creator "Harshvardhan J. Pandit, Rudy Jacob" ;
                      dct:description "Information that relates to an individual's TV viewing behavior, such as timestamps of channel change, duration of viewership, content consumed."@en ;
                      sw:term_status "proposed" .


###  http://w3.org/ns/dpv#Tattoo
dpv:Tattoo rdf:type owl:Class ;
           rdfs:subClassOf dpv:PhysicalCharacteristic ;
           dct:created "2019-04-04"^^xsd:date ;
           dct:creator "Elmar; Harshvardhan J. Pandit, Fajar" ;
           dct:date-accepted "2019-06-04"^^xsd:date ;
           dct:description "Information about an individual's tattoos"@en ;
           rdfs:isDefinedBy <https://enterprivacy.com/wp-content/uploads/2018/09/Categories-of-Personal-Information.pdf> ;
           sw:term_status "accepted" .


###  http://w3.org/ns/dpv#Tax
dpv:Tax rdf:type owl:Class ;
        rdfs:subClassOf dpv:Transactional ;
        dct:created "2019-04-04"^^xsd:date ;
        dct:creator "Elmar; Harshvardhan J. Pandit, Fajar" ;
        dct:date-accepted "2019-06-04"^^xsd:date ;
        dct:description "Information about financial tax e.g. tax records or tax due"@en ;
        rdfs:isDefinedBy <https://enterprivacy.com/wp-content/uploads/2018/09/Categories-of-Personal-Information.pdf> ;
        sw:term_status "accepted" .


###  http://w3.org/ns/dpv#TechnicalMeasure
dpv:TechnicalMeasure rdf:type owl:Class ;
                     rdfs:subClassOf dpv:TechnicalOrganisationalMeasure ;
                     dct:created "2019-04-04"^^xsd:date ;
                     dct:creator "Axel Polleres, Rob Brennan, Harshvardhan J. Pandit, Mark Lizar" ;
                     dct:date-accepted "2019-04-05"^^xsd:date ;
                     dct:description "Technical measures required/followed when processing data of the declared category"@en ;
                     rdfs:isDefinedBy "DPVCG" ;
                     sw:term_status "accepted" .


###  http://w3.org/ns/dpv#TechnicalOrganisationalMeasure
dpv:TechnicalOrganisationalMeasure rdf:type owl:Class ;
                                   dct:created "2019-04-04"^^xsd:date ;
                                   dct:creator "Bud Bruegger" ;
                                   dct:date-accepted "2019-04-05"^^xsd:date ;
                                   dct:description "Technical and organisational measures, for instance security measure, storage restrictions etc. required/followed when processing data of the declared category"@en ;
                                   rdfs:comment "Bud: rename according to GDPR: Technical/Organisational measures" ;
                                   rdfs:isDefinedBy "DPVCG" ;
                                   sw:term_status "accepted" .


###  http://w3.org/ns/dpv#TelephoneNumber
dpv:TelephoneNumber rdf:type owl:Class ;
                    rdfs:subClassOf dpv:Contact ;
                    dct:created "2019-04-04"^^xsd:date ;
                    dct:creator "Elmar; Harshvardhan J. Pandit, Fajar" ;
                    dct:date-accepted "2019-06-04"^^xsd:date ;
                    dct:description "Information about an individual's telephone number."@en ;
                    rdfs:isDefinedBy <https://enterprivacy.com/wp-content/uploads/2018/09/Categories-of-Personal-Information.pdf> ;
                    sw:term_status "accepted" .


###  http://w3.org/ns/dpv#ThirdParty
dpv:ThirdParty rdf:type owl:Class ;
               rdfs:subClassOf dpv:Recipient ;
               dct:created "2019-06-04"^^xsd:date ;
               dct:creator "Harshvardhan J. Pandit" ;
               dct:date-accepted "2019-06-04"^^xsd:date ;
               dct:description "‘third party’ means a natural or legal person, public authority, agency or body other than the data subject, controller, processor and persons who, under the direct authority of the controller or processor, are authorised to process personal data;"@en ;
               rdfs:isDefinedBy <https://eur-lex.europa.eu/eli/reg/2016/679/art_4/par_10/pnt_g/oj> ;
               sw:term_status "approved" .


###  http://w3.org/ns/dpv#Thought
dpv:Thought rdf:type owl:Class ;
            rdfs:subClassOf dpv:KnowledgeBelief ;
            dct:created "2019-04-04"^^xsd:date ;
            dct:creator "Elmar; Harshvardhan J. Pandit, Fajar" ;
            dct:date-accepted "2019-06-04"^^xsd:date ;
            dct:description "Information about an individual's thoughts"@en ;
            rdfs:isDefinedBy <https://enterprivacy.com/wp-content/uploads/2018/09/Categories-of-Personal-Information.pdf> ;
            sw:term_status "accepted" .


###  http://w3.org/ns/dpv#Tracking
dpv:Tracking rdf:type owl:Class ;
             rdfs:subClassOf dpv:PersonalDataCategory ;
             dct:created "2019-04-04"^^xsd:date ;
             dct:creator "Elmar; Harshvardhan J. Pandit, Fajar" ;
             dct:date-accepted "2019-06-04"^^xsd:date ;
             dct:description "Personal data that can be used to track an individual or used as an identifier e.g. location or email"@en ;
             rdfs:isDefinedBy <https://enterprivacy.com/wp-content/uploads/2018/09/Categories-of-Personal-Information.pdf> ;
             sw:term_status "accepted" .


###  http://w3.org/ns/dpv#Transaction
dpv:Transaction rdf:type owl:Class ;
                rdfs:subClassOf dpv:Transactional ;
                dct:created "2019-04-04"^^xsd:date ;
                dct:creator "Elmar; Harshvardhan J. Pandit, Fajar" ;
                dct:date-accepted "2019-06-04"^^xsd:date ;
                dct:description "Information about financial transactions e.g. bank transfers"@en ;
                rdfs:isDefinedBy <https://enterprivacy.com/wp-content/uploads/2018/09/Categories-of-Personal-Information.pdf> ;
                sw:term_status "accepted" .


###  http://w3.org/ns/dpv#Transactional
dpv:Transactional rdf:type owl:Class ;
                  rdfs:subClassOf dpv:Financial ;
                  dct:created "2019-04-04"^^xsd:date ;
                  dct:creator "Elmar; Harshvardhan J. Pandit, Fajar" ;
                  dct:date-accepted "2019-06-04"^^xsd:date ;
                  dct:description "Information about an individual’s purchasing, spending or income"@en ;
                  rdfs:isDefinedBy <https://enterprivacy.com/wp-content/uploads/2018/09/Categories-of-Personal-Information.pdf> ;
                  sw:term_status "accepted" .


###  http://w3.org/ns/dpv#Transfer
dpv:Transfer rdf:type owl:Class ;
             rdfs:subClassOf dpv:Processing ;
             dct:created "2019-04-04"^^xsd:date ;
             dct:date-accepted "2019-05-07"^^xsd:date ;
             dct:description "to move data from one place to another"@en ;
             rdfs:isDefinedBy <https://www.specialprivacy.eu/vocabs/processing> ;
             rdfs:seeAlso svpr:Transfer ;
             sw:term_status "accepted" .


###  http://w3.org/ns/dpv#Transform
dpv:Transform rdf:type owl:Class ;
              rdfs:subClassOf dpv:Processing ;
              dct:created "2019-04-04"^^xsd:date ;
              dct:date-accepted "2019-05-07"^^xsd:date ;
              dct:description "to change the form or nature of data"@en ;
              rdfs:isDefinedBy "DPVCG" ;
              sw:term_status "accepted" .


###  http://w3.org/ns/dpv#Transmit
dpv:Transmit rdf:type owl:Class ;
             rdfs:subClassOf dpv:Disclose ;
             dct:created "2019-04-04"^^xsd:date ;
             dct:date-accepted "2019-05-07"^^xsd:date ;
             dct:description "to send out data"@en ;
             rdfs:isDefinedBy "DPVCG" ;
             sw:term_status "accepted" .


###  http://w3.org/ns/dpv#UID
dpv:UID rdf:type owl:Class ;
        rdfs:subClassOf dpv:Identifying ;
        dct:created "2019-04-04"^^xsd:date ;
        dct:creator "Elmar; Harshvardhan J. Pandit, Fajar" ;
        dct:date-accepted "2019-06-04"^^xsd:date ;
        dct:description "An unique identifier used to identify an individual."@en ;
        rdfs:isDefinedBy <https://enterprivacy.com/wp-content/uploads/2018/09/Categories-of-Personal-Information.pdf> ;
        rdfs:seeAlso svd:UniqueId ;
        sw:term_status "accepted" .


###  http://w3.org/ns/dpv#Use
dpv:Use rdf:type owl:Class ;
        rdfs:subClassOf dpv:Processing ;
        dct:created "2019-04-04"^^xsd:date ;
        dct:date-accepted "2019-05-07"^^xsd:date ;
        dct:description "to use data"@en ;
        rdfs:isDefinedBy <https://eur-lex.europa.eu/eli/reg/2016/679/art_4/par_2/oj> ;
        sw:term_status "accepted" .


###  http://w3.org/ns/dpv#UserInterfacePersonalisation
dpv:UserInterfacePersonalisation rdf:type owl:Class ;
                                 rdfs:subClassOf dpv:ServicePersonalization ;
                                 dct:created "2018-12-10"^^xsd:date ;
                                 dct:creator "Harshvardhan J. Pandit, Javier Fernandez, Axel Polleres, Elmar Kiesling, Fajar Ekaputra, Simon Steyskal" ;
                                 dct:date-accepted "2019-04-05"^^xsd:date ;
                                 dct:description "Personalisation of interfaces presented to the user"@en ;
                                 rdfs:isDefinedBy <https://www.w3.org/community/dpvcg/wiki/Purposes_for_handling_Personal_Data#High-level_categories_.28to-be-discussed.29> ;
                                 sw:term_status "accepted" .


###  http://w3.org/ns/dpv#Username
dpv:Username rdf:type owl:Class ;
             rdfs:subClassOf dpv:Identifying ;
             dct:created "2019-04-04"^^xsd:date ;
             dct:creator "Elmar; Harshvardhan J. Pandit, Fajar" ;
             dct:date-accepted "2019-06-04"^^xsd:date ;
             dct:description "A username used to identify an individual."@en ;
             rdfs:isDefinedBy <https://enterprivacy.com/wp-content/uploads/2018/09/Categories-of-Personal-Information.pdf> ;
             sw:term_status "accepted" .


###  http://w3.org/ns/dpv#VoiceCommunicationRecording
dpv:VoiceCommunicationRecording rdf:type owl:Class ;
                                rdfs:subClassOf dpv:Communication ;
                                dct:created "2019-04-04"^^xsd:date ;
                                dct:creator "Elmar; Harshvardhan J. Pandit, Fajar, Axel Polleres" ;
                                dct:date-accepted "2019-06-04"^^xsd:date ;
                                dct:description "Recording of an individual's recorded communication (e.g. telephony, VoIP)"@en ;
                                rdfs:isDefinedBy <https://enterprivacy.com/wp-content/uploads/2018/09/Categories-of-Personal-Information.pdf> ;
                                sw:term_status "accepted" .


###  http://w3.org/ns/dpv#VoiceMail
dpv:VoiceMail rdf:type owl:Class ;
              rdfs:subClassOf dpv:Communication ;
              dct:created "2019-04-04"^^xsd:date ;
              dct:creator "Elmar; Harshvardhan J. Pandit, Fajar" ;
              dct:date-accepted "2019-06-04"^^xsd:date ;
              dct:description "Information about an individual's voice mail messages."@en ;
              rdfs:isDefinedBy <https://enterprivacy.com/wp-content/uploads/2018/09/Categories-of-Personal-Information.pdf> ;
              sw:term_status "accepted" .


###  http://w3.org/ns/dpv#Weight
dpv:Weight rdf:type owl:Class ;
           rdfs:subClassOf dpv:PhysicalCharacteristic ;
           dct:created "2019-04-04"^^xsd:date ;
           dct:creator "Elmar; Harshvardhan J. Pandit, Fajar" ;
           dct:date-accepted "2019-06-04"^^xsd:date ;
           dct:description "Information about an individual's physical weight"@en ;
           rdfs:isDefinedBy <https://enterprivacy.com/wp-content/uploads/2018/09/Categories-of-Personal-Information.pdf> ;
           sw:term_status "accepted" .


###  http://w3.org/ns/dpv#WorkHistory
dpv:WorkHistory rdf:type owl:Class ;
                rdfs:subClassOf dpv:Professional ;
                dct:created "2019-04-04"^^xsd:date ;
                dct:creator "Elmar; Harshvardhan J. Pandit, Fajar" ;
                dct:date-accepted "2019-06-04"^^xsd:date ;
                dct:description "Information about an individual's work history in a professional context"@en ;
                rdfs:isDefinedBy <https://enterprivacy.com/wp-content/uploads/2018/09/Categories-of-Personal-Information.pdf> ;
                sw:term_status "accepted" .


###  http://www.w3.org/2006/time#Instant
time:Instant rdf:type owl:Class .


###  http://www.w3.org/2006/time#TemporalEntity
time:TemporalEntity rdf:type owl:Class .


###  http://www.w3.org/ns/prov#Agent
prov:Agent rdf:type owl:Class .


#################################################################
#    Individuals
#################################################################

###  http://w3.org/ns/dpv#x1
dpv:x1 rdf:type owl:NamedIndividual ,
                dpv:PersonalDataHandling ;
       dpv:measureImplementedBy dpv:AccessControl .


###  Generated by the OWL API (version 4.5.9.2019-02-01T07:24:44Z) https://github.com/owlcs/owlapi
